format-version: 1.0
date: 18:06:2008 13:34
saved-by: annemaglia
auto-generated-by: OBO-Edit 1.101
default-namespace: amphibanat

[Term]
id: AAO:0000001
name: adipose_tissue
def: "Tissue that contains adipocytes, used for cushioning, thermal insulation, lubrication (primarily in the pericardium) and energy storage." [AAO:LAP]
is_a: AAO:0000099 ! connective_tissue_proper

[Term]
id: AAO:0000002
name: alary_cartilage
def: "Paired, cup-shaped cartilage that are dorsal to the septomaxillae and anterior to the oblique cartilage. The anterior, convex face of each alary cartilage is synchondrotically fused to the superior prenasal cartilage and the ventral edge is fused to the superior margin of the crista intermedia." [AAO:LAP]
related_synonym: "alinasal cartilage" []
related_synonym: "cartilago alaris" []
related_synonym: "cartilago alaris nasi" []
related_synonym: "cartilago cupullaris" []
related_synonym: "copula anterior" []
related_synonym: "naseflngelknorpel" []
related_synonym: "processus alaris" []
related_synonym: "second upper labial" []
relationship: part_of AAO:0000320 ! nasal_skeleton

[Term]
id: AAO:0000003
name: alary_process_of_premaxilla
def: "Dorsal process that extends toward the nasal bone. The posterior (inner) face of each alary process is concave and is invested dorsomedially by the superior prenasal cartilage and ventromedially by the inferior prenasal cartilage." [AAO:LAP]
related_synonym: "dorsal process of premaxilla" []
related_synonym: "pars dorsalis of premaxilla" []
related_synonym: "pars facialis of premaxilla" []
related_synonym: "pars frontalis of premaxilla" []
related_synonym: "pars prenasalis of premaxilla" []
related_synonym: "premaxillary spine" []
related_synonym: "processus ascendens of premaxilla" []
related_synonym: "processus frontalis of premaxilla" []
related_synonym: "processus nasalis of premaxilla" []
relationship: part_of AAO:0000461 ! premaxilla

[Term]
id: AAO:0000006
name: alveolar_foramen
def: "Foramen for the R. alveolaris of Nerve VII and the alveolar artery." [AAO:LAP]
is_a: AAO:0000273 ! lower_jaw_opening
synonym: "inferior dental foramen" RELATED[]

[Term]
id: AAO:0000007
name: anatomical_system

[Term]
id: AAO:0000010
name: angular
related_synonym: "postoperculare" []
related_synonym: "praearticulare" []
is_a: AAO:0000274 ! lower_jaw_skeleton

[Term]
id: AAO:0000012
name: angulosplenial_coronoid_process
def: "Point of insertion of the adductor mandibulae musculature." [AAO:LAP]
is_a: AAO:0000274 ! lower_jaw_skeleton

[Term]
id: AAO:0000013
name: animal_tissue
is_a: AAO:0000607 ! tissue

[Term]
id: AAO:0000015
name: anterior_maxillary_process
def: "Process that extends anteriorly from the planum triangulare and invests the medial face of the pars facialis of the maxilla." [AAO:LAP]
relationship: part_of AAO:0000320 ! nasal_skeleton

[Term]
id: AAO:0000016
name: anterior_nasal_wall
def: "Paired, vertical, and relatively straight plates that form the anterior limit of the nasal capsule." [AAO:LAP]
related_synonym: "prenasal wall" []
related_synonym: "solum anterius" []
relationship: part_of AAO:0000320 ! nasal_skeleton

[Term]
id: AAO:0000017
name: anterior_process_of_pars_palatina_of_maxilla
relationship: part_of AAO:0000413 ! pars_palatina_of_maxilla

[Term]
id: AAO:0000018
name: anterior_ramus_of_pterygoid
def: "In a triradiate pterygoid, the process that extends anteriorly towards the maxilla." [AAO:LAP]
related_synonym: "ramus maxillaris of pterygoid" []
relationship: part_of AAO:0000521 ! pterygoid

[Term]
id: AAO:0000020
name: anterolateral_process_of_frontoparietal
relationship: part_of AAO:0000207 ! frontoparietal

[Term]
id: AAO:0000022
name: antorbital_process
relationship: part_of AAO:0000400 ! pars_facialis_of_maxilla

[Term]
id: AAO:0000024
name: apertura_nasalis_externa
def: "Hole on the nasal capsule that connects the nasal cavity with the exterior." [AAO:LAP]
related_synonym: "external naris" []
related_synonym: "external nostril" []
related_synonym: "nostril" []
is_a: AAO:0000316 ! nasal_opening

[Term]
id: AAO:0000025
name: apertura_nasalis_interna
def: "Hole on the nasal capsule that connects the nasal and buccal cavites." [AAO:LAP]
related_synonym: "Choana" []
related_synonym: "internal naris" []
related_synonym: "internal nostril" []
is_a: AAO:0000316 ! nasal_opening

[Term]
id: AAO:0000027
name: areolar_connective_tissue
def: "Also known as loose connective tissue. A pliable, mesh-like tissue with a fluid matrix that functions to cushion and protect body organs." [AAO:LAP]
is_a: AAO:0000099 ! connective_tissue_proper

[Term]
id: AAO:0000028
name: articular
def: "Endochondral ossification of the posterior articular part of Meckel's cartilage." [AAO:LAP]
related_synonym: "angulaire" []
related_synonym: "angulare" []
related_synonym: "dermarticulare" []
related_synonym: "goniale" []
related_synonym: "operculo angulaire" []
relationship: part_of AAO:0000274 ! lower_jaw_skeleton

[Term]
id: AAO:0000031
name: ascending_process_of_palatoquadrate
related_synonym: "apophyse ascendens" []
related_synonym: "cartilage craniofacial" []
related_synonym: "oberste abteilung des zweiten visceralbogens" []
related_synonym: "pedicle" []
related_synonym: "pediculus" []
related_synonym: "processus ascendens of palatoquadrate" []
related_synonym: "schlafenflugelknorpel" []
relationship: part_of AAO:0000379 ! palatoquadrate

[Term]
id: AAO:0000032
name: auditory_muscles
is_a: AAO:0000107 ! cranial_muscles

[Term]
id: AAO:0000033
name: autonomic_nervous_system
is_a: AAO:0000429 ! peripheral_nervous_system

[Term]
id: AAO:0000034
name: axial_skeleton
def: "The axial skeleton is formed by the vertebral column, a metameric, semi-flexible, arched bar located in the dorsal part of the trunk, and is formed by a series of cartilaginous or bony vertebrae. It provides suspension for the appendicular skeleton and protection for the spinal nerve cord." [AAO:Pugener_and_Maglia_2008]
related_synonym: "spinal column" []
related_synonym: "vertebral column" []
relationship: part_of AAO:0000566 ! skeletal_system

[Term]
id: AAO:0000036
name: basal_process_of_palatoquadrate
def: "Process that extends medially from the ventromedial corner of the palatoquadrate cartilage and articulates or fuses to the anterior wall of the otic capsule via the basitrabecular process." [AAO:LAP]
related_synonym: "processus basalis" []
relationship: part_of AAO:0000379 ! palatoquadrate

[Term]
id: AAO:0000037
name: basicranial_fontanelle
def: "Ventral opening of the neurocranium." [AAO:LAP]
is_a: AAO:0000051 ! braincase_and_otic_capsule_opening

[Term]
id: AAO:0000038
name: basimandibulare
relationship: part_of AAO:0000274 ! lower_jaw_skeleton

[Term]
id: AAO:0000039
name: basioccipital
relationship: part_of AAO:0000052 ! braincase_and_otic_capsule_skeleton

[Term]
id: AAO:0000040
name: basisphenoid
def: "Endochondral ossification of the ventromedial portion of the braincase." [AAO:LAP]
relationship: part_of AAO:0000052 ! braincase_and_otic_capsule_skeleton

[Term]
id: AAO:0000041
name: bidders_organ
relationship: part_of AAO:0000624 ! urogenital_system

[Term]
id: AAO:0000042
name: blastoderm
is_a: AAO:0000138 ! embryonic_structure

[Term]
id: AAO:0000043
name: blastodisc
is_a: AAO:0000138 ! embryonic_structure

[Term]
id: AAO:0000044
name: blastomere
is_a: AAO:0000138 ! embryonic_structure

[Term]
id: AAO:0000045
name: blastopore
is_a: AAO:0000138 ! embryonic_structure

[Term]
id: AAO:0000046
name: blood
def: "Highly specialized circulating tissue consisting of several types of cells suspended in a fluid medium known as plasma." [AAO:LAP]
is_a: AAO:0000571 ! specialized_connective_tissue

[Term]
id: AAO:0000047
name: bone
def: "Also called osseous tissue, (Latin: os). Is a type of hard endoskeletal connective tissue found in many vertebrate animals. Bone is the main tissue of body organs; organs that support body structures, protect internal organs, (in conjunction with muscles) facilitate movement; and are involved with cell formation, calcium metabolism, and mineral storage." [AAO:LAP]
is_a: AAO:0000571 ! specialized_connective_tissue

[Term]
id: AAO:0000049
name: bottle_cells
is_a: AAO:0000138 ! embryonic_structure

[Term]
id: AAO:0000050
name: braincase_and_auditory_apparatus
def: "The part of the skull that encloses the brain and surrounds the inner ear." [AAO:LAP]
relationship: part_of AAO:0000109 ! cranial_skeleton

[Term]
id: AAO:0000051
name: braincase_and_otic_capsule_opening
is_a: AAO:0000050 ! braincase_and_auditory_apparatus

[Term]
id: AAO:0000052
name: braincase_and_otic_capsule_skeleton
is_a: AAO:0000050 ! braincase_and_auditory_apparatus

[Term]
id: AAO:0000053
name: buccal_cavity
relationship: part_of AAO:0000129 ! digestive_system

[Term]
id: AAO:0000054
name: buccopharyngeal_cavity
relationship: part_of AAO:0000541 ! respiratory_system

[Term]
id: AAO:0000057
name: canalis_semircularis_anterior
relationship: part_of AAO:0000420 ! pars_superior_of_labyrinth

[Term]
id: AAO:0000058
name: canalis_semircularis_posterior
relationship: part_of AAO:0000420 ! pars_superior_of_labyrinth

[Term]
id: AAO:0000059
name: capsular_process
def: "Narrow process of the skeletal support that projects forward." [AAO:LAP]
relationship: part_of AAO:0000565 ! skeletal_support_for_eminentia_olfactoria

[Term]
id: AAO:0000060
name: cartilage
def: "A type of dense connective tissue. It is composed of cells called chondrocytes which are dispersed in a firm gel-like ground substance, called the matrix. Cartilage is avascular (contains no blood vessels) and nutrients are diffused through the matrix. Cartilage is found in the joints, the rib cage, the ear, the nose, in the throat and between intervertebral disks. It makes up virtually the entire skeleton in chondrichthyes." [AAO:LAP]
is_a: AAO:0000571 ! specialized_connective_tissue

[Term]
id: AAO:0000061
name: cartilage_bridge
relationship: part_of AAO:0000320 ! nasal_skeleton

[Term]
id: AAO:0000068
name: cartilago_ectochoanalis
def: "Lateral cartilaginous border of the fenestra endochoanalis." [AAO:LAP]
relationship: part_of AAO:0000320 ! nasal_skeleton

[Term]
id: AAO:0000069
name: cartilago_infranarina
relationship: part_of AAO:0000320 ! nasal_skeleton

[Term]
id: AAO:0000074
name: cartilago_orbitalis
related_synonym: "dorsale randspange" []
relationship: part_of AAO:0000052 ! braincase_and_otic_capsule_skeleton

[Term]
id: AAO:0000078
name: cartilago_prootico-occipitalis
relationship: part_of AAO:0000052 ! braincase_and_otic_capsule_skeleton

[Term]
id: AAO:0000079
name: cartilago_retronarina
relationship: part_of AAO:0000320 ! nasal_skeleton

[Term]
id: AAO:0000080
name: caudal-sacral_region
def: "Region of the vertebral column posterior to the sacrum consisting of two to four vertebrae. The last of these vertebrae is distinguished by the possession of a well-developed haemal arch; it supports the posterior part of the cloaca and marks the posterior limit of the trunk." [AAO:Duellman_and_Treub_1994]
relationship: part_of AAO:0000699 ! vertebral_column_skeleton

[Term]
id: AAO:0000081
name: caudal_muscles
relationship: part_of AAO:0000307 ! muscular_system

[Term]
id: AAO:0000082
name: caudal_region
def: "Region of the vertebral column posterior to the caudal-sacral region, that may consists of two or three to more than 100 vertebrae. These vertebrae exhibit a gradual reduction in the sizes of their transverse processes and zygapophyses, but these structures are never entirely absent. All caudal vertebrae bear haemal arches." [AAO:Duellman_and_Trueb_1994]
related_synonym: "postsacral region" []
related_synonym: "tail region" []
relationship: part_of AAO:0000699 ! vertebral_column_skeleton

[Term]
id: AAO:0000085
name: cavum_inferius
def: "Accessory cavity located ventral to the cavum principale and cavum medius." [AAO:LAP]
is_a: AAO:0000314 ! nasal_cavity

[Term]
id: AAO:0000086
name: cavum_internasale
is_a: AAO:0000314 ! nasal_cavity

[Term]
id: AAO:0000087
name: cavum_medius
def: "Small accessory cavity located between the cavum principale and cavum inferius." [AAO:LAP]
is_a: AAO:0000314 ! nasal_cavity

[Term]
id: AAO:0000088
name: cavum_praenasale
is_a: AAO:0000314 ! nasal_cavity

[Term]
id: AAO:0000089
name: cavum_principale
def: "Largest and most dorsal of the nasal cavities." [AAO:LAP]
is_a: AAO:0000314 ! nasal_cavity

[Term]
id: AAO:0000090
name: central_nervous_system
relationship: part_of AAO:0000324 ! nervous_system

[Term]
id: AAO:0000091
name: cervical_muscles
relationship: part_of AAO:0000307 ! muscular_system

[Term]
id: AAO:0000092
name: cervical_region
def: "Anterior region of the vertebral column consisting of one to 19 or 20 vertebrae." [AAO:Duellman_and_Trueb_1994]
relationship: part_of AAO:0000699 ! vertebral_column_skeleton

[Term]
id: AAO:0000093
name: choana
def: "Opening between the nasal cavity and the nasopharynx." [AAO:LAP]
relationship: part_of AAO:0000541 ! respiratory_system

[Term]
id: AAO:0000094
name: chondrocranium
is_a: AAO:0000265 ! larval_structure

[Term]
id: AAO:0000095
name: cloaca
relationship: part_of AAO:0000624 ! urogenital_system

[Term]
id: AAO:0000098
name: connective_tissue
def: "One of the four types of tissue in traditional classifications. It is largely a category of exclusion rather than one with a precise definition, but there are certain characteristics shared by all or most tissues in this category, such as involvement in structure and support, derived from mesoderm, and characterized largely by the traits of non-living tissue." [AAO:LAP]
is_a: AAO:0000013 ! animal_tissue

[Term]
id: AAO:0000099
name: connective_tissue_proper
is_a: AAO:0000098 ! connective_tissue

[Term]
id: AAO:0000103
name: coronoid
relationship: part_of AAO:0000274 ! lower_jaw_skeleton

[Term]
id: AAO:0000104
name: coronoid_teeth
relationship: part_of AAO:0000126 ! dentition

[Term]
id: AAO:0000107
name: cranial_muscles
relationship: part_of AAO:0000307 ! muscular_system

[Term]
id: AAO:0000108
name: cranial_nerves
relationship: part_of AAO:0000324 ! nervous_system

[Term]
id: AAO:0000109
name: cranial_skeleton
def: "Bony structure that encases the central nervous system and the primary sense organs of sight, olfaction, hearing, and equilibrium." [AAO:Duellman_and_Trueb_1994]
relationship: part_of AAO:0000566 ! skeletal_system

[Term]
id: AAO:0000110
name: crista_contacta
def: "Thin, horizontal ridge that extends medially from the corpus of the septomaxilla; it lays on the lamina inferior." [AAO:LAP]
relationship: part_of AAO:0000645 ! corpus

[Term]
id: AAO:0000111
name: crista_dentalis_of_maxilla
relationship: part_of AAO:0000396 ! pars_dentalis_of_maxilla

[Term]
id: AAO:0000112
name: crista_dentalis_of_premaxilla
related_synonym: "dental ridge of premaxilla" []
relationship: part_of AAO:0000397 ! pars_dentalis_of_premaxilla

[Term]
id: AAO:0000113
name: crista_intermedia
def: "Paired, oblique plates of cartilage located ventral to the alary cartilages. The dorsomedial margin of each crista intermedia is fused to the transitional zone between the septum nasi and the tectum nasi, whereas the ventrolateral margin bears two laminae, the lamina superior and the lamina inferior." [AAO:LAP]
relationship: part_of AAO:0000320 ! nasal_skeleton

[Term]
id: AAO:0000115
name: crista_lateralis_of_premaxilla
relationship: part_of AAO:0000461 ! premaxilla

[Term]
id: AAO:0000116
name: crista_parotica
related_synonym: "processus muscularis capsulae auditivae" []
related_synonym: "processus squamosus" []
related_synonym: "tegmen tympani" []
relationship: part_of AAO:0000052 ! braincase_and_otic_capsule_skeleton

[Term]
id: AAO:0000117
name: crista_subnasalis
def: "Ventral crest of the paries nasi." [AAO:LAP]
related_synonym: "subnasal crest" []
relationship: part_of AAO:0000320 ! nasal_skeleton

[Term]
id: AAO:0000118
name: crista_supraorbitalis
def: "Short and blunt process that extends posteriorly from the posteromedial margin of the postnasal wall, on the anterodorsal corner of the orbit above the medial orbitonasal foramen." [AAO:LAP]
relationship: part_of AAO:0000320 ! nasal_skeleton

[Term]
id: AAO:0000119
name: cutaneous_muscles
relationship: part_of AAO:0000611 ! trunk_muscles

[Term]
id: AAO:0000121
name: dense_connective_tissue
def: "Also known as fibrous connective tissue. Forms ligaments and tendons and is characterized by densely packed collagen fibers that have great tensile strength." [AAO:LAP]
is_a: AAO:0000099 ! connective_tissue_proper

[Term]
id: AAO:0000124
name: dentary
def: "Ossified element of intramembranous origin that invests the lateral margin of the mentomeckelian bone and Meckel's cartilage, thus forming the lateral margin of the mandible." [AAO:LAP]
related_synonym: "dentale" []
related_synonym: "os dentale" []
related_synonym: "sur-angulaire" []
relationship: part_of AAO:0000274 ! lower_jaw_skeleton

[Term]
id: AAO:0000125
name: dentary_teeth
relationship: part_of AAO:0000126 ! dentition

[Term]
id: AAO:0000126
name: dentition
def: "Dentition refers to set of teeth, especially with regard to their number, kind, and arrangement, in the mouth." [AAO:LAP]
relationship: part_of AAO:0000109 ! cranial_skeleton

[Term]
id: AAO:0000128
name: dermis
is_a: AAO:0000239 ! integument

[Term]
id: AAO:0000129
name: digestive_system
is_a: AAO:0000007 ! anatomical_system

[Term]
id: AAO:0000130
name: digestive_system_glands
relationship: part_of AAO:0000129 ! digestive_system

[Term]
id: AAO:0000131
name: dilatatio_alaris
def: "Flange that extends ventrally from about the middle portion of the margo mandibularis." [AAO:LAP]
related_synonym: "ventral flange of anterior ramus of pterygoid" []
relationship: part_of AAO:0000280 ! margo_mandibularis_of_pterygoid

[Term]
id: AAO:0000132
name: dorsal_plate
relationship: part_of AAO:0000320 ! nasal_skeleton

[Term]
id: AAO:0000135
name: ductus_endolymphaticus
relationship: part_of AAO:0000141 ! endolymphatic_system

[Term]
id: AAO:0000136
name: ductus_perilymphaticus
relationship: part_of AAO:0000428 ! perilymphatic_system

[Term]
id: AAO:0000137
name: ectoderm
is_a: AAO:0000480 ! primary_germ_layer

[Term]
id: AAO:0000138
name: embryonic_structure

[Term]
id: AAO:0000139
name: endoderm
is_a: AAO:0000480 ! primary_germ_layer

[Term]
id: AAO:0000141
name: endolymphatic_system
relationship: part_of AAO:0000238 ! inner_ear

[Term]
id: AAO:0000142
name: epaxial_muscles
relationship: part_of AAO:0000611 ! trunk_muscles

[Term]
id: AAO:0000143
name: epidermis
is_a: AAO:0000239 ! integument

[Term]
id: AAO:0000144
name: epithelium
def: "One of the four types of tissue in traditional classifications. Tissues composed of layers of cells that cover organ surfaces such as surface of the skin and inner lining of digestive tract." [AAO:LAP]
is_a: AAO:0000013 ! animal_tissue

[Term]
id: AAO:0000145
name: esophagus
relationship: part_of AAO:0000129 ! digestive_system

[Term]
id: AAO:0000146
name: eustachian_canal
def: "Furrow on the ventral surface of the otic capsule, and occasionally also the parasphenoid, that houses the Eustachian tube." [AAO:LAP]
relationship: part_of AAO:0000052 ! braincase_and_otic_capsule_skeleton

[Term]
id: AAO:0000147
name: exoccipital
def: "Endochondral bone that forms the posterior end of the neurocranium and the margin of the foramen magnum. In addition, this bone contributes to the posteromedial portion of the otic capsule and forms the occipital condyle." [AAO:LAP]
related_synonym: "exoccipitale" []
related_synonym: "occipitale laterale" []
related_synonym: "opisthoticum" []
related_synonym: "pleurooccipitale" []
relationship: part_of AAO:0000052 ! braincase_and_otic_capsule_skeleton

[Term]
id: AAO:0000155
name: extremitas_anterior
def: "Large anterior outgrowth of the septomaxilla that is directed into the space between the alary cartilage and the lamina inferior." [AAO:LAP]
related_synonym: "anterior ramus" []
relationship: part_of AAO:0000556 ! septomaxilla

[Term]
id: AAO:0000156
name: eye_muscles
is_a: AAO:0000107 ! cranial_muscles

[Term]
id: AAO:0000157
name: fat_bodies
relationship: part_of AAO:0000624 ! urogenital_system

[Term]
id: AAO:0000160
name: fenestra_dorsalis_nasi
is_a: AAO:0000316 ! nasal_opening

[Term]
id: AAO:0000161
name: fenestra_endochoanalis
def: "Opening on the ventral aspect of the nasal capsule. It contains the apertura nasalis interna." [AAO:LAP]
related_synonym: "fenestra exochoanalis" []
is_a: AAO:0000316 ! nasal_opening

[Term]
id: AAO:0000162
name: fenestra_endonarina_communis
def: "Opening on the anterolateral aspect of the nasal capsule. It contains the apertura nasalis externa." [AAO:LAP]
related_synonym: "apertura nasalis externa" []
related_synonym: "fenestra narina" []
related_synonym: "narial fenestra" []
is_a: AAO:0000316 ! nasal_opening

[Term]
id: AAO:0000164
name: fenestra_lateralis_nasi
def: "Opening on the lateral side of the nasal capsule." [AAO:LAP]
related_synonym: "fenestra infraconchalis" []
related_synonym: "fenestra retronarina" []
is_a: AAO:0000316 ! nasal_opening

[Term]
id: AAO:0000166
name: fenestra_nasobasalis
def: "Small opening at the anterior tip of the nasal capsule, on the floor of the cavum inferius. It is located medially to the base of the inferior prenasal cartilage and serves for the passage of the ramus medialis narium and arteria orbitonasalis." [AAO:LAP]
related_synonym: "basal fenestra" []
related_synonym: "fenestra basalis nasi" []
related_synonym: "foramen apicale" []
related_synonym: "foramen epiphaniale" []
related_synonym: "nasobasal fenestra" []
is_a: AAO:0000316 ! nasal_opening

[Term]
id: AAO:0000167
name: fenestra_nasolateralis
def: "Elongated opening located on the lateral side of the nasal capsule." [AAO:LAP]
is_a: AAO:0000316 ! nasal_opening

[Term]
id: AAO:0000169
name: fenestra_ovalis
related_synonym: "fenestra vestibuli" []
related_synonym: "foramen ovale" []
is_a: AAO:0000051 ! braincase_and_otic_capsule_opening

[Term]
id: AAO:0000170
name: fenestra_precerebralis
is_a: AAO:0000316 ! nasal_opening

[Term]
id: AAO:0000171
name: fenestra_prechoanalis
def: "Large opening of the nasal floor anterior to the fenestra endochoanalis." [AAO:LAP]
is_a: AAO:0000316 ! nasal_opening

[Term]
id: AAO:0000177
name: flange_of_quadratojugal
relationship: part_of AAO:0000532 ! quadratojugal

[Term]
id: AAO:0000178
name: footplate_of_pars_media_plectri
def: "Independent, horizontal bar of cartilage located on the anterior part of the fenestra ovalis in front of the pars interna plectri." [AAO:LAP]
related_synonym: "fenestral plate" []
related_synonym: "interstapediale" []
related_synonym: "otostapes" []
related_synonym: "pars otica columellae" []
related_synonym: "pseudooperculum" []
relationship: part_of AAO:0000408 ! pars_media_plectri

[Term]
id: AAO:0000179
name: foramen_acusticum
related_synonym: "acoustic foramen" []
is_a: AAO:0000051 ! braincase_and_otic_capsule_opening

[Term]
id: AAO:0000180
name: foramen_acusticum_anterius
relationship: part_of AAO:0000179 ! foramen_acusticum

[Term]
id: AAO:0000181
name: foramen_acusticum_maius
relationship: part_of AAO:0000180 ! foramen_acusticum_anterius

[Term]
id: AAO:0000182
name: foramen_acusticum_minus
relationship: part_of AAO:0000180 ! foramen_acusticum_anterius

[Term]
id: AAO:0000183
name: foramen_acusticum_posterius
relationship: part_of AAO:0000179 ! foramen_acusticum

[Term]
id: AAO:0000185
name: foramen_endolymphaticum
related_synonym: "endolymphatic foramen" []
is_a: AAO:0000051 ! braincase_and_otic_capsule_opening

[Term]
id: AAO:0000189
name: foramen_orbitonasale_laterale
is_a: AAO:0000316 ! nasal_opening

[Term]
id: AAO:0000190
name: foramen_orbitonasale_mediale
related_synonym: "canalis orbitonasalis" []
related_synonym: "canalis orbitonasalis medialis" []
related_synonym: "foramen orbitonasale" []
is_a: AAO:0000316 ! nasal_opening

[Term]
id: AAO:0000192
name: foramen_perilymphaticum
is_a: AAO:0000051 ! braincase_and_otic_capsule_opening

[Term]
id: AAO:0000193
name: foramen_perilymphaticum_accessorium
relationship: part_of AAO:0000192 ! foramen_perilymphaticum

[Term]
id: AAO:0000194
name: foramen_perilymphaticum_superius
related_synonym: "foramen rotundum" []
related_synonym: "superior perilymphatic formaen" []
relationship: part_of AAO:0000192 ! foramen_perilymphaticum

[Term]
id: AAO:0000195
name: foramen_perilymphaticus_inferius
related_synonym: "foramen pro aquaeducto cochleae" []
related_synonym: "inferior perilymphatic foramen" []
relationship: part_of AAO:0000192 ! foramen_perilymphaticum

[Term]
id: AAO:0000199
name: fore_propodium
def: "Segment of the forearm corresponding to the humerus." [AAO:Duellman_and_Trueb_1994]
is_a: AAO:0000202 ! forelimb_skeleton

[Term]
id: AAO:0000200
name: fore_epipodium
def: "Segment of the forearm corresponding to the radius and ulna." [AAO:Duellman_and_Trueb_1994]
related_synonym: "antibrachium" []
is_a: AAO:0000202 ! forelimb_skeleton

[Term]
id: AAO:0000201
name: fore_mesopodium
def: "Segment of the forearm corresponding to the carpus. It consists of several elements that articulate with the radius and ulna at one end and the metacarpals at the other end." [AAO:Duellman_and_Trueb_1994]
is_a: AAO:0000202 ! forelimb_skeleton

[Term]
id: AAO:0000202
name: forelimb_skeleton
def: "Skeletal structure of the paired, anterior appendages." [AAO:LAP]
is_a: AAO:0000205 ! forelimb

[Term]
id: AAO:0000203
name: forelimb_muscles_proper
is_a: AAO:0000204 ! forelimb_muscles

[Term]
id: AAO:0000204
name: forelimb_muscles
relationship: part_of AAO:0000307 ! muscular_system

[Term]
id: AAO:0000205
name: forelimb
def: "Upper limb, which connects the manus with the pectoral girdle." [AAO:LAP]
relationship: part_of AAO:0000747 ! appendicular_skeleton

[Term]
id: AAO:0000206
name: frontal
relationship: part_of AAO:0000052 ! braincase_and_otic_capsule_skeleton

[Term]
id: AAO:0000207
name: frontoparietal
def: "Paired bone of intramembranous origin that roofs the braincase." [AAO:LAP]
related_synonym: "fronto-parietaux" []
related_synonym: "os fronto-parietale" []
related_synonym: "parietaux" []
related_synonym: "parietofrontal" []
relationship: part_of AAO:0000052 ! braincase_and_otic_capsule_skeleton

[Term]
id: AAO:0000208
name: frontoparietal_constriction
relationship: part_of AAO:0000207 ! frontoparietal

[Term]
id: AAO:0000209
name: frontoparietal_fontanelle
def: "Dorsal opening of the neurocranium." [AAO:LAP]
is_a: AAO:0000051 ! braincase_and_otic_capsule_opening

[Term]
id: AAO:0000211
name: germ_ring
is_a: AAO:0000138 ! embryonic_structure

[Term]
id: AAO:0000212
name: glands
is_a: AAO:0000239 ! integument

[Term]
id: AAO:0000213
name: gonad
relationship: part_of AAO:0000624 ! urogenital_system

[Term]
id: AAO:0000216
name: hind_epipodium
def: "Segment of the leg corresponding to the tibia and fibula." [AAO:Duellman_and_Trueb_1994]
is_a: AAO:0000217 ! hind_limb_skeleton

[Term]
id: AAO:0000217
name: hind_limb_skeleton
def: "Skeletal structure of the paired, posterior appendages." [AAO:LAP]
is_a: AAO:0000219 ! hind_limb

[Term]
id: AAO:0000218
name: hind_limb_muscles_proper
is_a: AAO:0000222 ! hindlimb_muscles

[Term]
id: AAO:0000219
name: hind_limb
def: "Lower limb, which connects the pes with the pelvic girdle." [AAO:LAP]
relationship: part_of AAO:0000747 ! appendicular_skeleton

[Term]
id: AAO:0000220
name: hind_mesopodium
def: "Segment of the leg corresponding to the tarsus. It consists of several elements that articulate with the tibia and fibula at one end and the metatarsals at the other end." [AAO:Duellman_and_Trueb_1994]
is_a: AAO:0000217 ! hind_limb_skeleton

[Term]
id: AAO:0000221
name: hind_metapodium
def: "Segment of the leg corresponding to the metatarsus, which articulates with the carpals at one end and with the phalanges at the other end." [AAO:Duellman_and_Trueb_1994]
is_a: AAO:0000217 ! hind_limb_skeleton

[Term]
id: AAO:0000222
name: hindlimb_muscles
relationship: part_of AAO:0000307 ! muscular_system

[Term]
id: AAO:0000224
name: hyobranchial_muscles
is_a: AAO:0000107 ! cranial_muscles

[Term]
id: AAO:0000225
name: hyoid_apparatus
def: "Apparatus located in the floor of the mouth, under the mandibular arcade. The apparatus consists of a central corpus and four pairs of processes. This apparatus serves as the site of insertion for a variety of muscles associated with movements of the tongue and as the origin of the m. hyoglossus." [AAO:Duellman_and_Trueb_1994]
related_synonym: "hyobranchial apparatus" []
relationship: part_of AAO:0000226 ! hyolaryngeal_complex

[Term]
id: AAO:0000226
name: hyolaryngeal_complex
def: "Complex formed by two units, the hyoid and laryngeal apparatuses, which are both derived from the larval hyobranchial skeleton." [AAO:LAP]
relationship: part_of AAO:0000566 ! skeletal_system

[Term]
id: AAO:0000228
name: hypaxial_muscles
relationship: part_of AAO:0000611 ! trunk_muscles

[Term]
id: AAO:0000229
name: hypoblast
is_a: AAO:0000138 ! embryonic_structure

[Term]
id: AAO:0000234
name: inferior_prenasal_cartilage
def: "Elongate cartilage that extends anteroventrally from the solum nasi to abut the ventral portion of the posterior aspect of the alary process of the premaxilla. It was first discribed by Wiedersheim in 1876." [AAO:LAP]
related_synonym: "inferior prenasal process" []
related_synonym: "processus prenasalis inferior" []
related_synonym: "processus prenasalis inferior lateralis" []
relationship: part_of AAO:0000320 ! nasal_skeleton

[Term]
id: AAO:0000237
name: infrarrostral_cartilage
relationship: part_of AAO:0000094 ! chondrocranium

[Term]
id: AAO:0000238
name: inner_ear
relationship: part_of AAO:0000052 ! braincase_and_otic_capsule_skeleton

[Term]
id: AAO:0000239
name: integument
is_a: AAO:0000007 ! anatomical_system

[Term]
id: AAO:0000246
name: intestines
relationship: part_of AAO:0000129 ! digestive_system

[Term]
id: AAO:0000247
name: jaw_muscles
is_a: AAO:0000107 ! cranial_muscles

[Term]
id: AAO:0000249
name: jugular_foramen
def: "Large foramen that houses the glossopharyngeal and vagus nerves and is located inside the condyloid fossa." [AAO:LAP]
is_a: AAO:0000051 ! braincase_and_otic_capsule_opening

[Term]
id: AAO:0000250
name: kidney
relationship: part_of AAO:0000624 ! urogenital_system

[Term]
id: AAO:0000253
name: lagena
relationship: part_of AAO:0000550 ! sacculus

[Term]
id: AAO:0000254
name: lamella_alaris
def: "Dorsal plate of the squamosal." [AAO:LAP]
related_synonym: "horizontal arm of squamosal" []
relationship: part_of AAO:0000574 ! squamosal

[Term]
id: AAO:0000255
name: lamina_anterior_of_pars_facialis
relationship: part_of AAO:0000400 ! pars_facialis_of_maxilla

[Term]
id: AAO:0000259
name: lamina_inferior
def: "Lateral expansion of the crista intermedia that serves as the floor of the cavum medium." [AAO:LAP]
related_synonym: "lamina inferior cristae intermediae" []
relationship: part_of AAO:0000320 ! nasal_skeleton

[Term]
id: AAO:0000260
name: lamina_nariochoanalis
def: "Free, dorsal margin of the lamina inferior." [AAO:LAP]
relationship: part_of AAO:0000320 ! nasal_skeleton

[Term]
id: AAO:0000262
name: lamina_orbitonasalis
def: "In the larva, structure that is fused to the wall of the braincase, lateral to the olfactory foramen, and separates the nasal capsule and orbit. In the adult frog it constitutes the ventral part of postnasal wall." [AAO:LAP]
relationship: part_of AAO:0000320 ! nasal_skeleton

[Term]
id: AAO:0000263
name: lamina_precerebralis
def: "Posterior face of septum nasi." [AAO:LAP]
relationship: part_of AAO:0000320 ! nasal_skeleton

[Term]
id: AAO:0000264
name: lamina_superior
def: "Lateral expansion of the crista intermedia that serves as the roof of the cavum medium." [AAO:LAP]
related_synonym: "Lamina superior cristae intermediae" []
relationship: part_of AAO:0000320 ! nasal_skeleton

[Term]
id: AAO:0000265
name: larval_structure

[Term]
id: AAO:0000267
name: laryngeal_apparatus
def: "Apparatus located between the lungs and the buccal cavity. This apparatus is composed of a pair of arytenoid cartilages that are supported by the cricoid ring." [AAO:LAP]
relationship: part_of AAO:0000226 ! hyolaryngeal_complex

[Term]
id: AAO:0000268
name: larynx
relationship: part_of AAO:0000541 ! respiratory_system

[Term]
id: AAO:0000269
name: lateral_line_system
is_a: AAO:0000555 ! sensory_system

[Term]
id: AAO:0000272
name: lower_jaw
def: "Inferior mandibular arch located on the anterior and lateral sides of the skull." [AAO:LAP]
relationship: part_of AAO:0000109 ! cranial_skeleton

[Term]
id: AAO:0000273
name: lower_jaw_opening
is_a: AAO:0000272 ! lower_jaw

[Term]
id: AAO:0000274
name: lower_jaw_skeleton
is_a: AAO:0000272 ! lower_jaw

[Term]
id: AAO:0000275
name: lungs
relationship: part_of AAO:0000541 ! respiratory_system

[Term]
id: AAO:0000277
name: mandibular_symphysis
relationship: part_of AAO:0000272 ! lower_jaw

[Term]
id: AAO:0000280
name: margo_mandibularis_of_pterygoid
def: "Ventrally directed margin that connects the anterior and posterior rami of the pterygoid." [AAO:LAP]
relationship: part_of AAO:0000521 ! pterygoid

[Term]
id: AAO:0000281
name: margo_orbitalis_of_maxilla
def: "Dorsal margin of the maxilla between the frontal and zygomatico-maxillary processes." [AAO:LAP]
relationship: part_of AAO:0000285 ! maxilla

[Term]
id: AAO:0000282
name: margo_orbitalis_of_pterygoid
def: "Margin that connects the anterior and medial rami of the pterygoid." [AAO:LAP]
relationship: part_of AAO:0000521 ! pterygoid

[Term]
id: AAO:0000283
name: margo_orbitalis_of_squamosal
def: "Anterior margin of the squamosal that takes part in the formation of the orbit." [AAO:LAP]
relationship: part_of AAO:0000254 ! lamella_alaris

[Term]
id: AAO:0000284
name: margo_tympanicus_of_pterygoid
def: "Margin that connects the posterior and medial rami of the pterygoid." [AAO:LAP]
relationship: part_of AAO:0000521 ! pterygoid

[Term]
id: AAO:0000285
name: maxilla
def: "Paired, intramembranous bone located on the lateral sides of the skull, posterior to the premaxillae." [AAO:LAP]
related_synonym: "os maxillaire" []
related_synonym: "os maxillare superior" []
related_synonym: "os maxillo-jugaux" []
relationship: part_of AAO:0000622 ! upper_jaw_skeleton

[Term]
id: AAO:0000287
name: maxillary_teeth
relationship: part_of AAO:0000126 ! dentition

[Term]
id: AAO:0000288
name: maxillopalatine
relationship: part_of AAO:0000622 ! upper_jaw_skeleton

[Term]
id: AAO:0000289
name: Meckel's_cartilage
def: "Paired, rod-shaped elements that extend the length of the mandible and lie between the dentaries and the angulosplenials." [AAO:LAP]
relationship: part_of AAO:0000274 ! lower_jaw_skeleton

[Term]
id: AAO:0000290
name: medial_inferior_prenasal_cartilage
relationship: part_of AAO:0000320 ! nasal_skeleton

[Term]
id: AAO:0000291
name: medial_orbitonasal_foramen
def: "Opening on the postnasal wall for the medial branch (= ramus medialis nasi) of the ophthalmicus nerve." [AAO:LAP]
is_a: AAO:0000316 ! nasal_opening

[Term]
id: AAO:0000292
name: medial_ramus_of_pterygoid
def: "In a triradiate pterygoid, the process that extends medially towards the otic capsule." [AAO:LAP]
related_synonym: "ramus interior of pterygoid" []
relationship: part_of AAO:0000521 ! pterygoid

[Term]
id: AAO:0000294
name: median_prenasal_process
def: "Anterior projection of the septum nasi that protrudes through the anterior nasal wall." [AAO:LAP]
related_synonym: "processus prenasalis medius" []
relationship: part_of AAO:0000559 ! septum_nasi

[Term]
id: AAO:0000295
name: median_symphysis
relationship: part_of AAO:0000620 ! upper_jaw

[Term]
id: AAO:0000298
name: mental_foramen
is_a: AAO:0000273 ! lower_jaw_opening

[Term]
id: AAO:0000301
name: mentomeckelian
def: "Paired, cylindrical, and small bones of endochondral origin that lie anteromedial to the anterior end of Meckel's cartilage. The precursors of the mentomeckelian bones are the larval infrarostral cartilages." [AAO:LAP]
relationship: part_of AAO:0000274 ! lower_jaw_skeleton

[Term]
id: AAO:0000303
name: mesethmoid
def: "Endochondral ossification of the anteromedial portion of the braincase." [AAO:LAP]
relationship: part_of AAO:0000052 ! braincase_and_otic_capsule_skeleton

[Term]
id: AAO:0000304
name: mesoderm
is_a: AAO:0000480 ! primary_germ_layer

[Term]
id: AAO:0000306
name: muscle_tissue
def: "One of the four types of tissue in traditional classifications. Tissue that contains cells with contractile filaments that move past each other and change the size of the cell. Muscle tissue also is separated into three distinct categories." [AAO:LAP]
is_a: AAO:0000013 ! animal_tissue

[Term]
id: AAO:0000307
name: muscular_system
is_a: AAO:0000007 ! anatomical_system

[Term]
id: AAO:0000309
name: narial_muscles
is_a: AAO:0000107 ! cranial_muscles

[Term]
id: AAO:0000311
name: naris
relationship: part_of AAO:0000541 ! respiratory_system

[Term]
id: AAO:0000312
name: nasal
def: "Paired bone of intramembranous origin that roofs the olfactory capsule." [AAO:LAP]
related_synonym: "frontaux anterieurs" []
related_synonym: "fronto-nasale" []
related_synonym: "fronto-nasaux" []
related_synonym: "nasale" []
related_synonym: "nasenstirnbein" []
related_synonym: "supraethmoid" []
relationship: part_of AAO:0000052 ! braincase_and_otic_capsule_skeleton

[Term]
id: AAO:0000313
name: nasal_capsule
def: "Structure that has both respiratory and olfactory functions and lies anterior to the braincase, in the foremost section of the cranium." [AAO:LAP]
relationship: part_of AAO:0000109 ! cranial_skeleton

[Term]
id: AAO:0000314
name: nasal_cavity
def: "Saclike space internal to the nasal capsule lined by respiratory and sensory epithelium and glandular tissue." [AAO:LAP]
is_a: AAO:0000313 ! nasal_capsule

[Term]
id: AAO:0000316
name: nasal_opening
is_a: AAO:0000313 ! nasal_capsule

[Term]
id: AAO:0000320
name: nasal_skeleton
def: "Structural framework that provides support to the nasal sacs and ducts." [AAO:LAP]
is_a: AAO:0000313 ! nasal_capsule

[Term]
id: AAO:0000323
name: nasopremaxilla
relationship: part_of AAO:0000622 ! upper_jaw_skeleton

[Term]
id: AAO:0000324
name: nervous_system
is_a: AAO:0000007 ! anatomical_system

[Term]
id: AAO:0000325
name: nervous_tissue
def: "One of the four types of tissue in traditional classifications. Cells forming the brain, spinal cord and peripheral nervous system." [AAO:LAP]
is_a: AAO:0000013 ! animal_tissue

[Term]
id: AAO:0000327
name: notochord
def: "Slender rod of fibrous connective tissue surrounding a core of fluid-filled cells of mesodermal origin; it lies above the gut and directly beneath the spinal cord. The notochord is present during early development and in a few cases it is retained through life; however, usually the notochord is replaced by the vertebral column." [AAO:Pugener_2002]
is_a: AAO:0000138 ! embryonic_structure

[Term]
id: AAO:0000329
name: oblique_cartilage
def: "Semi-circular cartilaginous sheet that lies lateral to the side of the septum nasi." [AAO:LAP]
related_synonym: "cartilago obliqua" []
related_synonym: "cartilago obliqua nasi" []
related_synonym: "cartilago obliquo" []
related_synonym: "dorsal process" []
related_synonym: "lamina obliqua" []
relationship: part_of AAO:0000320 ! nasal_skeleton

[Term]
id: AAO:0000330
name: occipital_condyle
relationship: part_of AAO:0000147 ! exoccipital

[Term]
id: AAO:0000332
name: oculomotor_foramen
is_a: AAO:0000051 ! braincase_and_otic_capsule_opening

[Term]
id: AAO:0000333
name: olfactory_foramen
is_a: AAO:0000316 ! nasal_opening

[Term]
id: AAO:0000334
name: olfactory_system
relationship: part_of AAO:0000555 ! sensory_system

[Term]
id: AAO:0000341
name: optic_fenestra
is_a: AAO:0000051 ! braincase_and_otic_capsule_opening

[Term]
id: AAO:0000342
name: optic_foramen
is_a: AAO:0000051 ! braincase_and_otic_capsule_opening

[Term]
id: AAO:0000343
name: orbit
is_a: AAO:0000051 ! braincase_and_otic_capsule_opening

[Term]
id: AAO:0000344
name: orbitonasal_foramen
def: "Foramen that forms a passage for one of the branches of the trigeminal nerve into the nasal region." [AAO:LAP]
is_a: AAO:0000051 ! braincase_and_otic_capsule_opening

[Term]
id: AAO:0000345
name: orbitosphenoid
def: "Endochondral ossification of the lateral sides of the braincase." [AAO:LAP]
relationship: part_of AAO:0000052 ! braincase_and_otic_capsule_skeleton

[Term]
id: AAO:0000346
name: organizer
is_a: AAO:0000138 ! embryonic_structure

[Term]
id: AAO:0000347
name: os_articulare
def: "Ossified posterior articular portion of Meckel's cartilage." [AAO:LAP]
relationship: part_of AAO:0000289 ! Meckel's_cartilage

[Term]
id: AAO:0000348
name: os_basale
relationship: part_of AAO:0000052 ! braincase_and_otic_capsule_skeleton

[Term]
id: AAO:0000362
name: other_muscles
relationship: part_of AAO:0000307 ! muscular_system

[Term]
id: AAO:0000363
name: otic_ligament
relationship: part_of AAO:0000379 ! palatoquadrate

[Term]
id: AAO:0000364
name: otic_plate_of_pterygoid
def: "Osseous expansion of the posterior and medial rami of the pterygoid." [AAO:LAP]
relationship: part_of AAO:0000521 ! pterygoid

[Term]
id: AAO:0000365
name: otic_process_of_palatoquadrate
relationship: part_of AAO:0000379 ! palatoquadrate

[Term]
id: AAO:0000367
name: otic_ramus_of_squamosal
def: "Ramus (process) that extends medially toward the otic capsule." [AAO:LAP]
related_synonym: "posterior ramus" []
related_synonym: "ramus paroticus" []
relationship: part_of AAO:0000254 ! lamella_alaris

[Term]
id: AAO:0000368
name: otoccipital
def: "Fused prootic and exoccipital bones." [AAO:LAP]
relationship: part_of AAO:0000052 ! braincase_and_otic_capsule_skeleton

[Term]
id: AAO:0000371
name: ovary
is_a: AAO:0000213 ! gonad

[Term]
id: AAO:0000372
name: palatine
def: "Sliver of bone that invest part of or all the posterior aspect of each antorbital plane." [AAO:LAP]
broad_synonym: "neopalatine" []
relationship: part_of AAO:0000052 ! braincase_and_otic_capsule_skeleton

[Term]
id: AAO:0000374
name: palatine_process_of_pars_palatina_of_premaxilla
related_synonym: "median palatal squame " []
relationship: part_of AAO:0000414 ! pars_palatina_of_premaxilla

[Term]
id: AAO:0000375
name: palatine_process_of_the_pars_facialis_of_the_maxilla
relationship: part_of AAO:0000400 ! pars_facialis_of_maxilla

[Term]
id: AAO:0000376
name: palatine_teeth
relationship: part_of AAO:0000126 ! dentition

[Term]
id: AAO:0000379
name: palatoquadrate
def: "Column of catilage, remnant in the adult of the larval palatoquadrate cartilage, that is located lateral or antero-lateral to the auditory capsule." [AAO:LAP]
relationship: part_of AAO:0000596 ! suspensorium

[Term]
id: AAO:0000380
name: palatoquadrate_articular_process
relationship: part_of AAO:0000379 ! palatoquadrate

[Term]
id: AAO:0000381
name: paranasal_commissure
def: "Cartilaginous bridge that extends posteriorly to the anterolateral corner of the posterior nasal wall." [AAO:LAP]
related_synonym: "commissura lateralis nasi" []
related_synonym: "connection between lamina nariochoanalis and postnasal wall" []
related_synonym: "processus lingularis" []
relationship: part_of AAO:0000320 ! nasal_skeleton

[Term]
id: AAO:0000384
name: parasagittal_crest
relationship: part_of AAO:0000207 ! frontoparietal

[Term]
id: AAO:0000385
name: parasphenoid
def: "Azygous, median bone of intramembranous origin that underlies the ventral surface of the braincase." [AAO:LAP]
related_synonym: "keilbein" []
related_synonym: "os parasphenoidale" []
related_synonym: "os sphenoideum" []
related_synonym: "parabasale" []
relationship: part_of AAO:0000052 ! braincase_and_otic_capsule_skeleton

[Term]
id: AAO:0000386
name: cultriform_process
def: "Process that extends anteriorly from the orbitotemporal region." [AAO:LAP]
related_synonym: "pars medialis" []
related_synonym: "rostrum" []
relationship: part_of AAO:0000385 ! parasphenoid

[Term]
id: AAO:0000387
name: subotic_ala
def: "Paired, lateral processes that, when present, support the otic capsules ventrally." [AAO:LAP]
related_synonym: "processus lateralis" []
relationship: part_of AAO:0000385 ! parasphenoid

[Term]
id: AAO:0000388
name: parasphenoid_teeth
relationship: part_of AAO:0000126 ! dentition

[Term]
id: AAO:0000389
name: paries_nasi
def: "Paired, elongate, ventrolaterally-orieted cartilaginous structures that extend to the premaxilla-maxilla articulation." [AAO:LAP]
relationship: part_of AAO:0000320 ! nasal_skeleton

[Term]
id: AAO:0000390
name: parietal
relationship: part_of AAO:0000052 ! braincase_and_otic_capsule_skeleton

[Term]
id: AAO:0000393
name: pars_amphibiorum
relationship: part_of AAO:0000550 ! sacculus

[Term]
id: AAO:0000394
name: pars_articularis_of_mandibular_arch
def: "Posterior end of Meckel's cartilage that forms the articular head of the mandibular arch." [AAO:LAP]
relationship: part_of AAO:0000289 ! Meckel's_cartilage

[Term]
id: AAO:0000395
name: pars_basilaris
relationship: part_of AAO:0000550 ! sacculus

[Term]
id: AAO:0000396
name: pars_dentalis_of_maxilla
def: "Tooth-bearing part of the maxilla." [AAO:LAP]
related_synonym: "crista dentalis" []
relationship: part_of AAO:0000285 ! maxilla

[Term]
id: AAO:0000397
name: pars_dentalis_of_premaxilla
def: "Tooth-bearing part of the premaxilla." [AAO:LAP]
relationship: part_of AAO:0000461 ! premaxilla

[Term]
id: AAO:0000399
name: pars_externa_plectri
related_synonym: "extracolumellare" []
related_synonym: "extrapediale" []
related_synonym: "extraplectral" []
related_synonym: "extrastapes" []
related_synonym: "hyostapes" []
related_synonym: "medio-stapedial" []
related_synonym: "pars quadrata columellae" []
relationship: part_of AAO:0000443 ! plectral_apparatus

[Term]
id: AAO:0000400
name: pars_facialis_of_maxilla
relationship: part_of AAO:0000285 ! maxilla

[Term]
id: AAO:0000401
name: pars_facialis_of_maxillopalatine
relationship: part_of AAO:0000288 ! maxillopalatine

[Term]
id: AAO:0000405
name: pars_inferior_of_labyrinth
relationship: part_of AAO:0000238 ! inner_ear

[Term]
id: AAO:0000406
name: pars_interna_plectri
def: "Plate-like structure that lies in the fenestra ovalis. It arises within the membrana opercularis in the posterior part of the fenestra." [AOO:LAP]
related_synonym: "operculum auris" []
related_synonym: "operculum fenestrae ovalis" []
relationship: part_of AAO:0000443 ! plectral_apparatus

[Term]
id: AAO:0000408
name: pars_media_plectri
relationship: part_of AAO:0000443 ! plectral_apparatus

[Term]
id: AAO:0000413
name: pars_palatina_of_maxilla
def: "Lingual ledge on the inner surface of the maxilla." [AAO:LAP]
related_synonym: "lamina horizontalis" []
relationship: part_of AAO:0000285 ! maxilla

[Term]
id: AAO:0000414
name: pars_palatina_of_premaxilla
def: "Lingual ledge on the inner surface of the premaxilla." [AAO:LAP]
relationship: part_of AAO:0000461 ! premaxilla

[Term]
id: AAO:0000420
name: pars_superior_of_labyrinth
relationship: part_of AAO:0000238 ! inner_ear

[Term]
id: AAO:0000422
name: pectoral_girdle
def: "Skeletal structure immediately behind the head attached to the vertebral column by muscles and supporting the forelimbs." [AAO:LAP]
related_synonym: "shoulder girdle" []
relationship: part_of AAO:0000747 ! appendicular_skeleton

[Term]
id: AAO:0000423
name: pectoral_girdle_muscles
relationship: part_of AAO:0000204 ! forelimb_muscles

[Term]
id: AAO:0000426
name: pelvic_girdle
def: "Skeletal structure by which the hind limbs are supported and attached to the vertebral column." [AAO:LAP]
relationship: part_of AAO:0000747 ! appendicular_skeleton

[Term]
id: AAO:0000427
name: pelvic_girdle_muscles
relationship: part_of AAO:0000222 ! hindlimb_muscles

[Term]
id: AAO:0000428
name: perilymphatic_system
relationship: part_of AAO:0000238 ! inner_ear

[Term]
id: AAO:0000429
name: peripheral_nervous_system
is_a: AAO:0000324 ! nervous_system

[Term]
id: AAO:0000430
name: pigment_cells
is_a: AAO:0000239 ! integument

[Term]
id: AAO:0000431
name: pila_antotica
relationship: part_of AAO:0000052 ! braincase_and_otic_capsule_skeleton

[Term]
id: AAO:0000432
name: pila_metoptica
relationship: part_of AAO:0000052 ! braincase_and_otic_capsule_skeleton

[Term]
id: AAO:0000433
name: pineal_foramen
relationship: part_of AAO:0000207 ! frontoparietal

[Term]
id: AAO:0000434
name: planum_antorbitale
relationship: part_of AAO:0000320 ! nasal_skeleton

[Term]
id: AAO:0000437
name: planum_conchale
relationship: part_of AAO:0000320 ! nasal_skeleton

[Term]
id: AAO:0000438
name: planum_internasale
relationship: part_of AAO:0000320 ! nasal_skeleton

[Term]
id: AAO:0000440
name: planum_terminale
def: "Vertical plate of cartilage that is fused posterodorsally to the oblique cartilage and anteriorly to the lamina inferior." [AAO:LAP]
related_synonym: "pars terminalis" []
related_synonym: "terminal plate" []
relationship: part_of AAO:0000320 ! nasal_skeleton

[Term]
id: AAO:0000441
name: planum_triangulare
def: "Cartilaginous, distal expansion of the lamina orbitonasalis that invests the pars facialis of the maxilla medially." [AAO:LAP]
relationship: part_of AAO:0000320 ! nasal_skeleton

[Term]
id: AAO:0000443
name: plectral_apparatus
def: "Complex sound-conducting anatomical structure." [AAO:LAP]
relationship: part_of AAO:0000052 ! braincase_and_otic_capsule_skeleton

[Term]
id: AAO:0000446
name: posterior_condyle
relationship: part_of AAO:0000515 ! pseudoangular

[Term]
id: AAO:0000448
name: posterior_maxillary_process
def: "Process that extends posteriorly from the planum triangulare and invests the maxilla laterally and the anterior ramus of the pterygoid medially." [AAO:LAP]
relationship: part_of AAO:0000320 ! nasal_skeleton

[Term]
id: AAO:0000449
name: posterior_maxillary_process_dorsal_process
relationship: part_of AAO:0000448 ! posterior_maxillary_process

[Term]
id: AAO:0000450
name: posterior_mental_process
relationship: part_of AAO:0000274 ! lower_jaw_skeleton

[Term]
id: AAO:0000451
name: posterior_ramus_of_pterygoid
def: "In a triradiate pterygoid, the process that extends posterolaterally towards the jaw articulation." [AAO:LAP]
relationship: part_of AAO:0000521 ! pterygoid

[Term]
id: AAO:0000453
name: posterolateral_vomerine_process
relationship: part_of AAO:0000633 ! vomer

[Term]
id: AAO:0000454
name: postnasal_wall
def: "Paired, anteriorly concave structures that form the posterior limit of nasal capsule. It consists of two parts: a ventral piece, the lamina orbitonasalis, and a dorsal plate that is part of the tectum nasi." [AAO:LAP]
relationship: part_of AAO:0000320 ! nasal_skeleton

[Term]
id: AAO:0000458
name: prearticular
def: "Osseous element of intramembranous origin that extends along the lingual margin of Meckel's cartilage." [AAO:LAP]
relationship: part_of AAO:0000274 ! lower_jaw_skeleton

[Term]
id: AAO:0000459
name: prearticular_coronoid_process
def: "Point of insertion of the masticatory musculature." [AAO:LAP]
relationship: part_of AAO:0000458 ! prearticular

[Term]
id: AAO:0000460
name: prefrontal
relationship: part_of AAO:0000052 ! braincase_and_otic_capsule_skeleton

[Term]
id: AAO:0000461
name: premaxilla
def: "Paired, intramembranous bones located at the anterior end of the skull; they form the anterior-most segment of the maxillary arch." [AAO:LAP]
related_synonym: "intermaxillaire" []
related_synonym: "premaxillary" []
relationship: part_of AAO:0000622 ! upper_jaw_skeleton

[Term]
id: AAO:0000464
name: premaxillary_teeth
relationship: part_of AAO:0000126 ! dentition

[Term]
id: AAO:0000467
name: preorbital_process_of_the_pars_facialis_of_the_maxilla
relationship: part_of AAO:0000400 ! pars_facialis_of_maxilla

[Term]
id: AAO:0000468
name: presumptive_blood
is_a: AAO:0000479 ! presumptive_structure

[Term]
id: AAO:0000469
name: presumptive_central_nervous_system
is_a: AAO:0000477 ! presumptive_nervous_system

[Term]
id: AAO:0000470
name: presumptive_ectoderm
is_a: AAO:0000479 ! presumptive_structure

[Term]
id: AAO:0000471
name: presumptive_endoderm
is_a: AAO:0000479 ! presumptive_structure

[Term]
id: AAO:0000472
name: presumptive_enteric_nervous_system
is_a: AAO:0000477 ! presumptive_nervous_system

[Term]
id: AAO:0000473
name: presumptive_epidermis
is_a: AAO:0000475 ! presumptive_integument

[Term]
id: AAO:0000474
name: presumptive_hypochord
is_a: AAO:0000479 ! presumptive_structure

[Term]
id: AAO:0000475
name: presumptive_integument
is_a: AAO:0000479 ! presumptive_structure

[Term]
id: AAO:0000476
name: presumptive_mesoderm
is_a: AAO:0000479 ! presumptive_structure

[Term]
id: AAO:0000477
name: presumptive_nervous_system
is_a: AAO:0000479 ! presumptive_structure

[Term]
id: AAO:0000478
name: presumptive_notochord
is_a: AAO:0000479 ! presumptive_structure

[Term]
id: AAO:0000479
name: presumptive_structure
is_a: AAO:0000138 ! embryonic_structure

[Term]
id: AAO:0000480
name: primary_germ_layer
is_a: AAO:0000138 ! embryonic_structure

[Term]
id: AAO:0000486
name: processus_ascendens_plectri
def: "Cartilaginous or ligamentous connection between the pars externa plectri and the crista parotica." [AAO:LAP]
related_synonym: "laterohyale" []
related_synonym: "processus ascendens columellae" []
related_synonym: "processus dorsalis columellae" []
related_synonym: "processus superior columellae" []
related_synonym: "suprastapediale" []
relationship: part_of AAO:0000399 ! pars_externa_plectri

[Term]
id: AAO:0000492
name: processus_infrafenestralis
def: "Posterior part of the corpus of the septomaxilla; the posterior surface of the processus infrafenestralis is in contact with the oblique cartilage." [AAO:LAP]
related_synonym: "dorsal crest" []
relationship: part_of AAO:0000645 ! corpus

[Term]
id: AAO:0000493
name: processus_internus
relationship: part_of AAO:0000515 ! pseudoangular

[Term]
id: AAO:0000494
name: processus_lingualis_of_pterygoid
def: "Dorsolateral process of the of the medial ramus of the pterygoid." [AAO:LAP]
relationship: part_of AAO:0000292 ! medial_ramus_of_pterygoid

[Term]
id: AAO:0000500
name: processus_posterior_of_maxilla
def: "Posterior, toothless portion of the maxilla by which it usually comes in contact with the quadratojugal." [AAO:LAP]
relationship: part_of AAO:0000285 ! maxilla

[Term]
id: AAO:0000505
name: processus_pterygoideus_of_maxilla
def: "Posterior end of the pars palatina of the maxilla that is in contact with the anterior ramus of the pterygoid." [AAO:LAP]
relationship: part_of AAO:0000413 ! pars_palatina_of_maxilla

[Term]
id: AAO:0000509
name: processus_suprafenestralis
relationship: part_of AAO:0000645 ! corpus

[Term]
id: AAO:0000512
name: processus_zygomatico-maxillaris
def: "Posterodorsal extension of the maxilla by which it establishes contact with the squamosal." [AAO:LAP]
relationship: part_of AAO:0000285 ! maxilla

[Term]
id: AAO:0000514
name: prootic
def: "Paired, endochondral bones that form the lateral borders of the posterior portion of the braincase and the dorsal, anterior, and lateral walls of the otic capsules." [AAO:LAP]
relationship: part_of AAO:0000052 ! braincase_and_otic_capsule_skeleton

[Term]
id: AAO:0000515
name: pseudoangular
relationship: part_of AAO:0000274 ! lower_jaw_skeleton

[Term]
id: AAO:0000516
name: pseudobasal_process
relationship: part_of AAO:0000379 ! palatoquadrate

[Term]
id: AAO:0000518
name: pseudodentary
relationship: part_of AAO:0000274 ! lower_jaw_skeleton

[Term]
id: AAO:0000519
name: pseudodentary_teeth
relationship: part_of AAO:0000126 ! dentition

[Term]
id: AAO:0000521
name: pterygoid
def: "Palatal bones of intramembranous origin that lie anterior to the otic capsules, lateral to the orbits, and medial to the maxillae." [AAO:LAP]
related_synonym: "pterygoidien" []
relationship: part_of AAO:0000596 ! suspensorium

[Term]
id: AAO:0000523
name: pterygoid_process_of_palatoquadrate
def: "Process that extends anteriorly from the anterolateral margin of the palatoquadrate and articulates or synchondrotically fuses to the posterior end of the posterior maxillary process." [AAO:LAP]
relationship: part_of AAO:0000379 ! palatoquadrate

[Term]
id: AAO:0000524
name: pterygoquadrate
relationship: part_of AAO:0000596 ! suspensorium

[Term]
id: AAO:0000525
name: quadrate_bone
def: "Ossified pars articularis of the palatoquadrate cartilage." [AAO:LAP]
relationship: part_of AAO:0000596 ! suspensorium

[Term]
id: AAO:0000527
name: quadrate_process_of_palatoquadrate
relationship: part_of AAO:0000379 ! palatoquadrate

[Term]
id: AAO:0000532
name: quadratojugal
def: "Paired intramembranous bones that completes the maxillary arch posteriorly; they appear at the end of, or just after, metamorphosis." [AAO:LAP]
related_synonym: "jugau" []
related_synonym: "os jugale" []
related_synonym: "quadratjochbeine" []
related_synonym: "quadrato-jugals" []
related_synonym: "quadrato-maxillare" []
related_synonym: "quadratojugale" []
related_synonym: "tympano maleaux" []
relationship: part_of AAO:0000622 ! upper_jaw_skeleton

[Term]
id: AAO:0000538
name: recessus_fenestrae_ovalis
relationship: part_of AAO:0000428 ! perilymphatic_system

[Term]
id: AAO:0000539
name: recessus_marsupiatus_of_premaxilla
relationship: part_of AAO:0000461 ! premaxilla

[Term]
id: AAO:0000540
name: recessus_vaginiformis
relationship: part_of AAO:0000285 ! maxilla

[Term]
id: AAO:0000541
name: respiratory_system
is_a: AAO:0000007 ! anatomical_system

[Term]
id: AAO:0000542
name: reticular_connective_tissue
def: "Network of reticular fibres (fine collagen) that form a soft skeleton to support the lymphoid organs (lymph nodes, bone marrow, and spleen)." [AAO:LAP]
is_a: AAO:0000099 ! connective_tissue_proper

[Term]
id: AAO:0000543
name: retroarticular_process
def: "Point of insertion of the m. interhuoideus posterior." [AAO:LAP]
relationship: part_of AAO:0000515 ! pseudoangular

[Term]
id: AAO:0000545
name: rib
def: "Endochondral, rodlike element that articulates with the transverse process and parapophysis (double-headed rib), or with the transverse process only (single-headed rib); it extends into the body wall and provides a site for muscle attachment." [AAO:Pugener_2002]
related_synonym: "dorsal rib" []
relationship: part_of AAO:0000699 ! vertebral_column_skeleton

[Term]
id: AAO:0000547
name: rostral_process
relationship: part_of AAO:0000312 ! nasal

[Term]
id: AAO:0000550
name: sacculus
relationship: part_of AAO:0000405 ! pars_inferior_of_labyrinth

[Term]
id: AAO:0000551
name: saccus_endolymphaticus
relationship: part_of AAO:0000141 ! endolymphatic_system

[Term]
id: AAO:0000552
name: sacrum
def: "Enlarged vertebra with transverse processes (diapophyses), and ocassionally ribs, that are modified and elaborated for support of the pelvic girdle." [AAO:Duellman_and_Trueb_1994]
relationship: part_of AAO:0000724 ! sacral_region

[Term]
id: AAO:0000555
name: sensory_system
relationship: part_of AAO:0000324 ! nervous_system

[Term]
id: AAO:0000556
name: septomaxilla
def: "Paired, intramembranous bones located within the nasal capsules and embedded in the nasal cartilages; it is pierced by the ductus nasolacrimalis." [AAO:LAP]
related_synonym: "internasale" []
related_synonym: "intranasal" []
related_synonym: "lacrimale" []
related_synonym: "le cornet" []
related_synonym: "nariale" []
related_synonym: "nasale" []
related_synonym: "os internasale" []
related_synonym: "os nariale" []
related_synonym: "septomaxillary" []
related_synonym: "turbinale" []
relationship: part_of AAO:0000320 ! nasal_skeleton

[Term]
id: AAO:0000559
name: septum_nasi
def: "Medial, vertical plate that separates the nasal capsules." [AAO:LAP]
relationship: part_of AAO:0000320 ! nasal_skeleton

[Term]
id: AAO:0000560
name: septum_semicircularium_anterior
relationship: part_of AAO:0000238 ! inner_ear

[Term]
id: AAO:0000561
name: septum_semicircularium_laterale
relationship: part_of AAO:0000238 ! inner_ear

[Term]
id: AAO:0000562
name: septum_semircularium_posterior
relationship: part_of AAO:0000238 ! inner_ear

[Term]
id: AAO:0000563
name: seydels_palatal_process
relationship: part_of AAO:0000068 ! cartilago_ectochoanalis

[Term]
id: AAO:0000565
name: skeletal_support_for_eminentia_olfactoria
def: "Elevation of the dorsal surface of the solum nasi medial to the fenestra endochoanalis that provides support for the eminentia olfactoria." [AAO:LAP]
relationship: part_of AAO:0000320 ! nasal_skeleton

[Term]
id: AAO:0000566
name: skeletal_system
def: "System that provides physical support to the organism." [AAO:LAP]
is_a: AAO:0000007 ! anatomical_system

[Term]
id: AAO:0000569
name: solum_nasi
def: "Unpaired, horizontal plate that forms the floor of the nasal capsule." [AAO:LAP]
related_synonym: "nasal floor" []
related_synonym: "planum basale" []
relationship: part_of AAO:0000320 ! nasal_skeleton

[Term]
id: AAO:0000570
name: spatium_sacculare
relationship: part_of AAO:0000428 ! perilymphatic_system

[Term]
id: AAO:0000571
name: specialized_connective_tissue
is_a: AAO:0000098 ! connective_tissue

[Term]
id: AAO:0000572
name: sphenethmoid
def: "Azygous, endochondral bone that houses the anterior portion of the brain." [AAO:LAP]
relationship: part_of AAO:0000052 ! braincase_and_otic_capsule_skeleton

[Term]
id: AAO:0000573
name: splenial
relationship: part_of AAO:0000274 ! lower_jaw_skeleton

[Term]
id: AAO:0000574
name: squamosal
def: "Paired, intramembranous bones that lie at the posterolateral margins of the skull. These bones are composed of three rami that give the squamosals their characteristic T shape." [AAO:LAP]
related_synonym: "os squamosum" []
related_synonym: "os tympanicum" []
related_synonym: "paraquadratum" []
related_synonym: "squamosum" []
related_synonym: "supratemporale" []
related_synonym: "supratemporo-squamosum" []
related_synonym: "temporo-mastoidien" []
related_synonym: "tympanique" []
relationship: part_of AAO:0000596 ! suspensorium

[Term]
id: AAO:0000579
name: stomach
relationship: part_of AAO:0000129 ! digestive_system

[Term]
id: AAO:0000580
name: stylus_of_pars_media_plectri
related_synonym: "columella auris" []
related_synonym: "columellare" []
related_synonym: "interstapediale" []
related_synonym: "mediostapediale" []
related_synonym: "mesostapediale" []
related_synonym: "os columellare" []
related_synonym: "os intermedium" []
related_synonym: "stapes" []
related_synonym: "stelidium" []
related_synonym: "stilus columellare" []
relationship: part_of AAO:0000408 ! pars_media_plectri

[Term]
id: AAO:0000581
name: sulcus_dentalis_of_maxilla
def: "Groove located between the pars dentalis and the bases of the maxillary teeth." [AAO:LAP]
relationship: part_of AAO:0000285 ! maxilla

[Term]
id: AAO:0000582
name: sulcus_dentalis_of_premaxilla
relationship: part_of AAO:0000461 ! premaxilla

[Term]
id: AAO:0000583
name: sulcus_for_Meckels_cartilage
relationship: part_of AAO:0000012 ! angulosplenial_coronoid_process

[Term]
id: AAO:0000586
name: superior_prenasal_cartilage
def: "Paired, elongate cartilages that extend anteroventrally to abut the dorsomedial margin of the posterior face of the alary process of the premaxilla. The function of these cartilages is to transmit the movement of the premaxilla to the alary cartilages during the closure of the apertura nasalis externa." [AAO:LAP]
relationship: part_of AAO:0000320 ! nasal_skeleton

[Term]
id: AAO:0000587
name: supraangular
relationship: part_of AAO:0000274 ! lower_jaw_skeleton

[Term]
id: AAO:0000588
name: supraoccipital
relationship: part_of AAO:0000052 ! braincase_and_otic_capsule_skeleton

[Term]
id: AAO:0000590
name: supraorbital_flange
relationship: part_of AAO:0000207 ! frontoparietal

[Term]
id: AAO:0000591
name: suprasphenoid
def: "Endochondral ossification of the dorsomedial portion of the braincase." [AAO:LAP]
relationship: part_of AAO:0000052 ! braincase_and_otic_capsule_skeleton

[Term]
id: AAO:0000596
name: suspensorium
def: "Apparatus located toward the posterolateral end of the skull, at the level of the anterior margin of the otic capsule that suspends and braces the jaw against the skull." [AAO:LAP]
relationship: part_of AAO:0000109 ! cranial_skeleton

[Term]
id: AAO:0000597
name: symphysis_maxillaris
relationship: part_of AAO:0000620 ! upper_jaw

[Term]
id: AAO:0000599
name: taenia_tecti_marginalis
relationship: part_of AAO:0000052 ! braincase_and_otic_capsule_skeleton

[Term]
id: AAO:0000601
name: tectum_nasi
def: "Roof of the nasal capsule." [AAO:LAP]
relationship: part_of AAO:0000320 ! nasal_skeleton

[Term]
id: AAO:0000602
name: tectum_synoticum
relationship: part_of AAO:0000052 ! braincase_and_otic_capsule_skeleton

[Term]
id: AAO:0000605
name: tentacular_foramen
is_a: AAO:0000621 ! upper_jaw_opening

[Term]
id: AAO:0000606
name: testis
is_a: AAO:0000213 ! gonad

[Term]
id: AAO:0000607
name: tissue

[Term]
id: AAO:0000610
name: trochlear_foramen
is_a: AAO:0000051 ! braincase_and_otic_capsule_opening

[Term]
id: AAO:0000611
name: trunk_muscles
relationship: part_of AAO:0000307 ! muscular_system

[Term]
id: AAO:0000612
name: trunk_region
def: "Region of the vertebral column between the atlas and the sacrum consisting of seven to 285 vertebrae." [AAO:Duellman_and_Trueb_1994]
related_synonym: "presacral region" []
related_synonym: "thoracolumbar region" []
relationship: part_of AAO:0000699 ! vertebral_column_skeleton

[Term]
id: AAO:0000615
name: tympanic_annulus
def: "Funnel-like ring structure located lateral to the ventral ramus of the squamosal, beneath the skin; it provides support to the tympanic membrane." [AAO:LAP]
related_synonym: "annulus tympanicus" []
related_synonym: "processus basilaris" []
related_synonym: "tympanic ring" []
relationship: part_of AAO:0000443 ! plectral_apparatus

[Term]
id: AAO:0000619
name: tympanosquamosal
def: "Central, funnel-shaped, ossified portion of the tympanic annulus fused to the squamosal bone." [AAO:LAP]
relationship: part_of AAO:0000596 ! suspensorium

[Term]
id: AAO:0000620
name: upper_jaw
def: "Superior maxillary arch located on the anterior and lateral sides of the skull." [AAO:LAP]
relationship: part_of AAO:0000109 ! cranial_skeleton

[Term]
id: AAO:0000621
name: upper_jaw_opening
is_a: AAO:0000620 ! upper_jaw

[Term]
id: AAO:0000622
name: upper_jaw_skeleton
is_a: AAO:0000620 ! upper_jaw

[Term]
id: AAO:0000623
name: urinary_bladder
relationship: part_of AAO:0000624 ! urogenital_system

[Term]
id: AAO:0000624
name: urogenital_system
is_a: AAO:0000007 ! anatomical_system

[Term]
id: AAO:0000625
name: utriculus
relationship: part_of AAO:0000420 ! pars_superior_of_labyrinth

[Term]
id: AAO:0000628
name: ventral_ramus_of_squamosal
def: "Longest of the three squamosal rami; it invests the dorsolateral margin of the palatoquadrate. The distal end of the ventral ramus invests the quadrate and articulates with the quadratojugal." [AAO:LAP]
related_synonym: "processus posterolateralis" []
relationship: part_of AAO:0000574 ! squamosal

[Term]
id: AAO:0000629
name: ventrolateral_process_of_palatoquadrate
relationship: part_of AAO:0000094 ! chondrocranium

[Term]
id: AAO:0000631
name: vestibuloauditory_system
is_a: AAO:0000555 ! sensory_system

[Term]
id: AAO:0000632
name: visual_system
is_a: AAO:0000555 ! sensory_system

[Term]
id: AAO:0000633
name: vomer
def: "Paired, palatal bones of intramembranous origin that lie ventral to the olfactory region and help to floor the nasal capsules ." [AAO:LAP]
related_synonym: "praevomer" []
related_synonym: "prevomer" []
relationship: part_of AAO:0000052 ! braincase_and_otic_capsule_skeleton

[Term]
id: AAO:0000634
name: vomerine_canal
relationship: part_of AAO:0000633 ! vomer

[Term]
id: AAO:0000635
name: vomerine_teeth
relationship: part_of AAO:0000126 ! dentition

[Term]
id: AAO:0000637
name: Wolffian_duct
relationship: part_of AAO:0000624 ! urogenital_system

[Term]
id: AAO:0000639
name: zygomatic_ramus_of_squamosal
def: "Ramus (process) that forms part of the posterior margin of the orbit." [AAO:LAP]
relationship: part_of AAO:0000254 ! lamella_alaris

[Term]
id: AAO:0000640
name: arcus_praeoccipitalis
def: "Skeletal structure that separates the inferior and superior perilymphatic foramina." [AAO:LAP]
relationship: part_of AAO:0000052 ! braincase_and_otic_capsule_skeleton

[Term]
id: AAO:0000641
name: mandibular_teeth
relationship: part_of AAO:0000126 ! dentition

[Term]
id: AAO:0000642
name: maxillopalatine_teeth
relationship: part_of AAO:0000126 ! dentition

[Term]
id: AAO:0000643
name: nasolarimal_duct
related_synonym: "canalis nasolacrimalis" []
related_synonym: "ductus nasolacrimalis" []
related_synonym: "nasal duct" []
is_a: AAO:0000316 ! nasal_opening

[Term]
id: AAO:0000644
name: processus_lingularis
def: "Rod-shaped process that extends caudally from the inferior edge of the planum terminale." [AAO:LAP]
related_synonym: "lingular process" []
relationship: part_of AAO:0000320 ! nasal_skeleton

[Term]
id: AAO:0000645
name: corpus
def: "Basal part of the septomaxilla." [AAO:LAP]
related_synonym: "pars horizontalis" []
relationship: part_of AAO:0000556 ! septomaxilla

[Term]
id: AAO:0000646
name: margo_libera
def: "Anterior, rounded portion of the corpus of the septomaxilla." [AAO:LAP]
relationship: part_of AAO:0000645 ! corpus

[Term]
id: AAO:0000647
name: crista_interna
def: "Sharp ridge that extends medially from the basal part of the processus infrafenestralis; it separates the diverticulum proncipale from the diverticulum medium." [AAO:LAP]
relationship: part_of AAO:0000492 ! processus_infrafenestralis

[Term]
id: AAO:0000648
name: crista_praeopercularis
def: "Synchondrotic or synostotic connection between the footplate of the pars media plectri and the ventral margin of the fenestra ovalis." [AAO:LAP]
relationship: part_of AAO:0000408 ! pars_media_plectri

[Term]
id: AAO:0000649
name: anterior_process_of_vomer
def: "Process that extends anterolaterally toward the maxilla-premaxilla articulation." [AAO:LAP]
relationship: part_of AAO:0000633 ! vomer

[Term]
id: AAO:0000650
name: processus_frontalis
def: "Anterio portion of the maxilla that may contact the nasal and take part in the formation of a groove for the nasolacrimal duct." [AAO:LAP]
related_synonym: "processus praeorbitalis of the pars facialis" []
relationship: part_of AAO:0000285 ! maxilla

[Term]
id: AAO:0000651
name: lamina_anterior_of_maxilla
def: "Most anterior part of the maxilla, which is in contact with the premaxilla." [AAO:LAP]
relationship: part_of AAO:0000285 ! maxilla

[Term]
id: AAO:0000652
name: fossa_maxillaris
def: "Depression lacated on the inner surface of the maxilla between the palatine process and the pars palatina." [AAO:LAP]
relationship: part_of AAO:0000285 ! maxilla

[Term]
id: AAO:0000653
name: pars_glenoidalis_of_quadratojugal
def: "Portion of the quadratojugal that makes contact dorsally with the distal portion of the squamosal." [AAO:LAP]
relationship: part_of AAO:0000532 ! quadratojugal

[Term]
id: AAO:0000654
name: pars_jugalis
def: "Anterior part of the quadratojugal that is in contact with the processus posterior of the maxilla." [AAO:LAP]
relationship: part_of AAO:0000532 ! quadratojugal

[Term]
id: AAO:0000655
name: processus_dorsalis
def: "Dorsal process of the lamella alaris located at the anterior end of the margo orbitalis; a narrow ligament that runs from the frontoparietal is attached to it." [AAO:LAP]
relationship: part_of AAO:0000254 ! lamella_alaris

[Term]
id: AAO:0000656
name: processus_posterodorsalis
def: "Posterior process of the lamella alaris." [AAO:LAP]
relationship: part_of AAO:0000254 ! lamella_alaris

[Term]
id: AAO:0000657
name: dentigerous_ process
def: "Tooth-bearing process of the vomer." [AAO:LAP]
related_synonym: "torus dentigerous" []
relationship: part_of AAO:0000633 ! vomer

[Term]
id: AAO:0000658
name: prechoanal_process
def: "Process that extends laterally from the anterior process; its bifurcation from the postchoanal process occurs at the level of the dentigerous process." [AAO:LAP]
related_synonym: "processus choanalis anterior" []
relationship: part_of AAO:0000633 ! vomer

[Term]
id: AAO:0000659
name: postchoanal_process
def: "Process that extends laterally from the anterior process; its bifurcation from the prechoanal process occurs at the level of the dentigerous process." [AAO:LAP]
related_synonym: "processus choanalis posterior" []
relationship: part_of AAO:0000633 ! vomer

[Term]
id: AAO:0000660
name: margo_choanalis
def: "Margin between the prechoanal and postchoanal process. It bounds the fenestra endochoanalis." [AAO:LAP]
relationship: part_of AAO:0000633 ! vomer

[Term]
id: AAO:0000661
name: crista_vomeri
def: "Ridge on the dorsal surface of the vomer that runs from the anterior to the postchoanal processes of the vomer; it takes part in the fixation of the bone to the lateral margin of the solum nasi." [AAO:LAP]
relationship: part_of AAO:0000633 ! vomer

[Term]
id: AAO:0000662
name: processus_posterior
def: "Posterior projection of the median part of the parsphenoid, which may extend over the posterior margins of the subotic alae." [AAO:LAP]
relationship: part_of AAO:0000385 ! parasphenoid

[Term]
id: AAO:0000663
name: parahyoid
relationship: part_of AAO:0000225 ! hyoid_apparatus

[Term]
id: AAO:0000664
name: hyoid_plate
def: "Azygous or paired bone that occurs on the ventral surface of the hyoid plate." [AAO:LAP]
relationship: part_of AAO:0000225 ! hyoid_apparatus

[Term]
id: AAO:0000665
name: hyobranchial_skeleton
is_a: AAO:0000265 ! larval_structure

[Term]
id: AAO:0000666
name: ceratohyal
def: "Paired elements that lie ventral to the hypobranchials and curve dorsally from their medial articulation with basibranchial toward the suspensorium." [AAO:Duellman_and_Trueb_1994]
related_synonym: "ceratohyale" []
related_synonym: "hyale" []
related_synonym: "hyoid" []
related_synonym: "keratohyale" []
related_synonym: "zungenbeinknorpel" []
relationship: part_of AAO:0000665 ! hyobranchial_skeleton

[Term]
id: AAO:0000667
name: pars_reuniens
def: "Area of fusion of the ceratohyals." [AAO:LAP]
relationship: part_of AAO:0000665 ! hyobranchial_skeleton

[Term]
id: AAO:0000668
name: hypoglossal_sinus
relationship: part_of AAO:0000225 ! hyoid_apparatus

[Term]
id: AAO:0000669
name: hyale
relationship: part_of AAO:0000225 ! hyoid_apparatus

[Term]
id: AAO:0000670
name: anterior_process_of_hyoid_apparatus
relationship: part_of AAO:0000225 ! hyoid_apparatus

[Term]
id: AAO:0000671
name: anterolateral_process_of_hyoid_plate
def: "Processes that flank the hyales laterally and extend anterolaterally from the anterolateral margin of the hyoid plate. They are formed as a result of new cartilaginous growth lateral to the basibranchial." [AAO:Rocek_2003]
related_synonym: "processus alaris" []
related_synonym: "processus anterolateralis" []
related_synonym: "processus lateralis anterior" []
relationship: part_of AAO:0000664 ! hyoid_plate

[Term]
id: AAO:0000672
name: posterolateral_process
def: "Paired processes that extend posterolaterally from the posterolateral margin of the hyoid plate. These processes are formed as a result of new cartilaginous growth lateral to the basibranchial and hypobranchial plate." [AAO:LAP]
relationship: part_of AAO:0000664 ! hyoid_plate

[Term]
id: AAO:0000673
name: posteromedial_process
def: "Cartilaginous, paired processes that extend posterolaterally from the posterior margin of the hyoid plate. These processes invest the laryngeal apparatus and are ossified in the adult." [AAO:LAP]
related_synonym: "cornua posteriores" []
related_synonym: "hyoid" []
relationship: part_of AAO:0000664 ! hyoid_plate

[Term]
id: AAO:0000674
name: arytenoid_cartilage
def: "Paired, anteroposteriorly elongated cartilages that are associated with the vocal cords. These cartilages are medially separated and hemispherical, and their concave side faces ventromedially." [AAO:Maglia_et_al_2007, AAO:Rocek_2003]
related_synonym: "cartilago arytaenoidea" []
relationship: part_of AAO:0000267 ! laryngeal_apparatus

[Term]
id: AAO:0000675
name: cricoid_cartilage
def: "Cartilaginous ring that provides support for the arytenoid cartilages. Its ventral part is bent posteriorly to form a V." [AAO:Maglia_et_al_2003, AAO:Rocek_2003]
related_synonym: "cartilago cricoidea" []
related_synonym: "cartilago cricotrachealis" []
relationship: part_of AAO:0000267 ! laryngeal_apparatus

[Term]
id: AAO:0000676
name: bronchial_process
def: "Paired processes that extend posteroventrally from the anterolateral margins of the cricoid ring." [AAO:Maglia_et_al_2007]
related_synonym: "processus trachealis" []
relationship: part_of AAO:0000675 ! cricoid_cartilage

[Term]
id: AAO:0000677
name: lateral_process
relationship: part_of AAO:0000675 ! cricoid_cartilage

[Term]
id: AAO:0000678
name: esophageal_process
def: "Median process located on the posterior end of the cricoid cartilage." [AAO:Rocek_2003]
related_synonym: "spina oesophagea" []
relationship: part_of AAO:0000675 ! cricoid_cartilage

[Term]
id: AAO:0000679
name: humerus
def: "Paired, elongate, cylindrical bones of endochondral origin that extend from the pectoral girdle to the elbows." [AAO:Maglia_et_al_1994]
relationship: part_of AAO:0000199 ! fore_propodium

[Term]
id: AAO:0000680
name: manubrium
def: "Proximal section of the hyale." [AAO:Rocek_1993]
related_synonym: "processus anteriores" []
relationship: part_of AAO:0000669 ! hyale

[Term]
id: AAO:0000681
name: hyoid_apparatus_opening
is_a: AAO:0000225 ! hyoid_apparatus

[Term]
id: AAO:0000682
name: hyoid_apparatus_skeleton
is_a: AAO:0000225 ! hyoid_apparatus

[Term]
id: AAO:0000683
name: sinus_nervi_hypoglossi
def: "Depression that houses the hypoglossus nerve and is located between the anterolateral process and the proximal part of the hyale." [AAO:Rocek_2003]
is_a: AAO:0000681 ! hyoid_apparatus_opening

[Term]
id: AAO:0000684
name: hyoid_bone
def: "Paired processes that extend posterolaterally from the posterior margin of the hyoid plate. These processes are the ossified posteromedial processes and invest the laryngeal apparatus." [AAO:Rocek_2003]
related_synonym: "hyoid" []
related_synonym: "os postero-mediale" []
related_synonym: "ossa thyroidea" []
relationship: part_of AAO:0000664 ! hyoid_plate

[Term]
id: AAO:0000685
name: foramen_nervi_hypoglossi
def: "Foramen that houses the hypoglossus nerve and is located between the anterolateral process and the proximal part of the hyale." [AAO:Rocek_2003]
related_synonym: "foramen laterale" []
is_a: AAO:0000681 ! hyoid_apparatus_opening

[Term]
id: AAO:0000686
name: basibranchial
def: "Medial element to which other parts of the hyoid apparatus are attached." [AAO:Duellman_and_Trueb_1994]
related_synonym: "copula I" []
relationship: part_of AAO:0000682 ! hyoid_apparatus_skeleton

[Term]
id: AAO:0000687
name: processus_confluens
def: "Strip of cartilage that forms the lateral margin of the foramen nervi hypoglossi." [AAO:Rocek_2003]
related_synonym: "processus alaris" []
relationship: part_of AAO:0000669 ! hyale

[Term]
id: AAO:0000688
name: prominentia_apicalis_dorsalis
def: "Anterior end of the arytenoid cartilage." [AAO:Rocek_2003]
related_synonym: "prominentia apicalis anterior" []
relationship: part_of AAO:0000674 ! arytenoid_cartilage

[Term]
id: AAO:0000689
name: prominentia_apicalis_ventralis
def: "Posterior (cardiac) end of the arytenoid cartilage." [AAO:Rocek_2003]
related_synonym: "prominentia apicalis posterior" []
relationship: part_of AAO:0000674 ! arytenoid_cartilage

[Term]
id: AAO:0000690
name: wrisbergi_cartilage
def: "Independent cartilage that may occur dorsal or anterior to the prominentiae apicales dorsales of the arytenoid cartilages." [AAO:Rocek_2003]
related_synonym: "cartilago apicalis intermedia" []
related_synonym: "cartilago apicalis seu cartilago santoriniana" []
relationship: part_of AAO:0000267 ! laryngeal_apparatus

[Term]
id: AAO:0000691
name: vertebra
def: "Main component of the vertebral column. It consists of two essential parts, a dorsal neural arch and a ventral centrum." [AAO:Pugener_and_Maglia_2008]
relationship: part_of AAO:0000699 ! vertebral_column_skeleton

[Term]
id: AAO:0000692
name: pedicel
def: "Paired stalks located dorsolateral to the vertebral centrum that provide support to the lateral margins of the neural arch laminae." [AAO:LAP]
relationship: part_of AAO:0000691 ! vertebra

[Term]
id: AAO:0000693
name: neural_canal
def: "Canal formed by the vertebral centra ventrally, the pedicels laterally, and the neural arches dorsally that encloses and protects the spinal cord." [AAO:LAP]
related_synonym: "foramen vertebrale" []
related_synonym: "spinal canal" []
is_a: AAO:0000700 ! vertebral_column_opening

[Term]
id: AAO:0000694
name: atlantal_cotyle
def: "Anterior, single or paired concave facets for articulation with the condyle(s) of the urostyle." [AAO:Francis_1934]
related_synonym: "cavitas glenoidalis" []
relationship: part_of AAO:0000709 ! atlas

[Term]
id: AAO:0000695
name: neural_arch_lamina
def: "Paired plates that form the neural arch. The lateral margin of each lamina rests dorsal to the superior end of the pedicel, and the medial end fuses to the medial end of the opposite lamina." [AAO:Pugener_and_Maglia_2008]
relationship: part_of AAO:0000725 ! neural_arch

[Term]
id: AAO:0000696
name: posterior_intervertebral_notch
def: "Indentation on the anterior margin of the pedicel. When two vertebrae articulate, the anterior notch of one vertebra and the posterior notch of the other create a bilateral intervertebral space." [AAO:LAP]
relationship: part_of AAO:0000691 ! vertebra

[Term]
id: AAO:0000697
name: centrum
def: "Cylindrical body of bone, round or oval in cross section, which functionally replaces the notochord." [AAO:Duellman_and_Trueb_2008]
related_synonym: "corpus" []
relationship: part_of AAO:0000691 ! vertebra

[Term]
id: AAO:0000698
name: transverse_process
def: "Projections on each side of the vertebra from the point where the neural arch lamina joins the pedicel for the articulation with the head of a single-headed rib or the upper head of a double-headed rib. Also called diapophyses. They provide surfaces for the attachment of muscles. In anurans, the term transverse process is used in reference to the processes associated with the presacral and postsacral vertebrae." [AAO:Pugener_2002, AAO:Pugener_and_Maglia_2008, AAO:Trueb_1973]
relationship: part_of AAO:0000691 ! vertebra

[Term]
id: AAO:0000699
name: vertebral_column_skeleton
is_a: AAO:0000034 ! axial_skeleton

[Term]
id: AAO:0000700
name: vertebral_column_opening
is_a: AAO:0000034 ! axial_skeleton

[Term]
id: AAO:0000701
name: intervertebral_space
def: "Space formed by the anterior and posterior intervertebral notches. The intervertebral spaces accommodate the spinal nerves as they emerge from the spinal canal." [AAO:LAP]
related_synonym: "intervertebral space" []
is_a: AAO:0000700 ! vertebral_column_opening

[Term]
id: AAO:0000702
name: postzygapophysis
def: "Paired processes at the caudal end of the neural arch. The articular facets of the postzygapophyses face lateroventrally and articulate with the dorsomedially facing facets of the prezygapophyses of the succeeding vertebra." [AAO:LAP]
related_synonym: "processus obliquus posterior" []
is_a: AAO:0000710 ! zygapophysis

[Term]
id: AAO:0000703
name: prezygapophysis
def: "Paired processes at the cephalic end of the neural arch. The articular facets of the prezygapophyses face dorsomedially and articulate with the lateroventrally facing facets of the postzygapophyses of the preceding vertebra." [AAO:Pugener_and_Maglia_2008]
related_synonym: "processus obliquus anterior" []
is_a: AAO:0000710 ! zygapophysis

[Term]
id: AAO:0000704
name: anterior_intervertebral_notch
def: "Indentation on the posterior margin of the pedicel. When two vertebrae articulate, the anterior notch of one vertebra and the posterior notch of the other create a bilateral intervertebral space." [AAO:LAP]
relationship: part_of AAO:0000691 ! vertebra

[Term]
id: AAO:0000705
name: neural_spine
def: "Elaboration of the mid-dorsal keel into a posterior or posterolateral process." [AAO:Pugener_and_Maglia_2008]
related_synonym: "processus spinosus" []
relationship: part_of AAO:0000735 ! mid-dorsal_keel

[Term]
id: AAO:0000706
name: diapophysis
def: "Paired processes that arise near the midpoint of the neural arch lamina, for the attachment of the tuberculum of two-headed ribs. Also called transverse processes. In anurans, the term diapophysis is used in reference to the modified transverse processes of the sacral vertebra elaborated for support of the pelvic girdle." [AAO:Duellman_and_Trueb_1994, AAO:Pugener_2002]
relationship: part_of AAO:0000691 ! vertebra

[Term]
id: AAO:0000707
name: pleurapophysis
def: "Paired processes that represent the rib attachments to the vertebra plus the ribs." [AAO:Duellman_and_Trueb_1994]
relationship: part_of AAO:0000691 ! vertebra

[Term]
id: AAO:0000708
name: parapophysis
def: "Paired processes, which arise near the dorsolateral part of the vertebral centrum, for the attachment of the capitulum of two-headed ribs." [AAO:Duellman_and_Trueb_1994]
relationship: part_of AAO:0000691 ! vertebra

[Term]
id: AAO:0000709
name: atlas
def: "First postcranial vertebra, which is modified anteriorly to articulate with the skull." [AAO:Duellman_and_Trueb_1994]
related_synonym: "presacral I" []
relationship: part_of AAO:0000092 ! cervical_region

[Term]
id: AAO:0000710
name: zygapophysis
def: "Paired processes at the cephalic and caudal ends of the neural arch. They function as interlocking structures between adjacent vertebrae, and limit dorsoventral flexion and lateral movement of the column in the trunk region." [AAO:Pugener_and_Maglia_2008]
related_synonym: "processus articularis" []
relationship: part_of AAO:0000691 ! vertebra

[Term]
id: AAO:0000711
name: procoelous
def: "Holochordal vertebral centra that are concave anteriorly and convex posteriorly; they bear a condyle on the posterior end for the articulation with the posterior adjacent vertebral centrum, forming a ball-and-socket joint that allows extensive motion in most directions." [AAO:Pugener_2002, AAO:Trueb_1973]
is_a: AAO:0000697 ! centrum

[Term]
id: AAO:0000712
name: opisthocoelous
def: "Ectochordal or stegochordal vertebral centra that are convex anteriorly and concave posteriorly; they bear a condyle on the anterior end for the articulation with the posterior adjacent vertebral centrum, forming a ball-and-socket joint that allows extensive motion in most directions." [AAO:Pugener_2002, AAO:Trueb_1973]
is_a: AAO:0000697 ! centrum

[Term]
id: AAO:0000713
name: epichordal
def: "Vertebral centrum that originates from ossification of the dorsal portion of the perichordal tube; the resulting element tends to be depressed in cross section." [AAO:Kluge_and_Farris_1969]
is_a: AAO:0000697 ! centrum

[Term]
id: AAO:0000714
name: perichordal
def: "Vertebral centrum that originates from ossification of the entire perichordal tube; the resulting element is cylindrical in cross section and may have an open (notochord retained) or solid center." [AAO:Kluge_and_Farris_1969]
is_a: AAO:0000697 ! centrum

[Term]
id: AAO:0000715
name: heterocoelous
def: "Vertebral centrum that bears saddle-shaped articular surfaces at both ends, having a convexity in the right-left axis and a concavity in the dorsoventral axis. This morphology allows great lateral and vertical flexion." [AAO:LAP]
is_a: AAO:0000697 ! centrum

[Term]
id: AAO:0000716
name: acoelous
def: "Vertebral centrum with flat ends. Between successive vertebrae there is a fibrocartilaginous intervertebral body with a gel-like core, the nucleus pulposus, which is derived from the embryonic notochord. Acoelous vertebrae seem especially suited to receive and distribute compressive forces within the vertebral column." [AAO:LAP]
is_a: AAO:0000697 ! centrum

[Term]
id: AAO:0000717
name: amphicoelous
def: "Ectochordal, biconcave or terminally flat vertebral centrum. This design seems to allow limited motion in most directions. An intervertebral body (which may or may not be independent from the adjacent centra) fills the cavity between successive centra. The intervertebral body usually is formed by soft material that may be derived, at least in part, from the embryonic notochord." [AAO:Pugener_2002, AAO:Trueb_1973]
is_a: AAO:0000697 ! centrum

[Term]
id: AAO:0000718
name: ectochordal
def: "Spool-shaped vertebral centrum with an open center in which the notochord lies." [AAO:Griffiths_1959]
is_a: AAO:0000697 ! centrum

[Term]
id: AAO:0000719
name: holochordal
def: "Spool-shaped vertebral centrum with a solid center. All traces of the notochord dissapear." [AAO:Griffiths_1959]
is_a: AAO:0000697 ! centrum

[Term]
id: AAO:0000720
name: stegochordal
def: "Vertebral centrum that is depressed dorsoventrally and solid. All traces of the notochord dissapear." [AAO:Griffiths_1959]
is_a: AAO:0000697 ! centrum

[Term]
id: AAO:0000721
name: odontoid_process
def: "Anterior process located between the atlantal cotyles that projects into the foramen magnum of the skull and bears facets that articulate with the lateral walls of the foramen." [AAO:Duellman_and_Trueb_1994]
related_synonym: "tuberculum interglenoideum" []
relationship: part_of AAO:0000709 ! atlas

[Term]
id: AAO:0000722
name: tuberculum
def: "Dorsal head of a bicapitate rib. It articulates with the diapophysis." [AAO:Duellman_and_Trueb_1994]
relationship: part_of AAO:0000545 ! rib

[Term]
id: AAO:0000723
name: capitulum_of_rib
def: "Ventral head of a bicapitate rib. It articulates with the parapophysis." [AAO:Duellman_and_Trueb_1994]
relationship: part_of AAO:0000545 ! rib

[Term]
id: AAO:0000724
name: sacral_region
def: "Region of the vertebral column represented by one or two vertebrae." [AAO:Duellman_and_Trueb_1994]
relationship: part_of AAO:0000699 ! vertebral_column_skeleton

[Term]
id: AAO:0000725
name: neural_arch
def: "Bony arch perched on the vertebral centrum; successive arches enclose the neural canal that surrounds and protects the spinal cord dorsally." [AAO:Pugener_2002]
related_synonym: "carina neuralis" []
relationship: part_of AAO:0000691 ! vertebra

[Term]
id: AAO:0000726
name: haemal_arch
def: "Bony canal attached to the ventral surface or the vertebral centrum that encloses and protects the caudal artery and vein ventrally. The arch consists of right and left halves, which are fused ventrally to give a V- or Y-shape to the ventral aspect of the vertebra." [AAO:Pugener_2002]
related_synonym: "ventral arch" []
relationship: part_of AAO:0000691 ! vertebra

[Term]
id: AAO:0000727
name: haemal_arch_lamina
def: "Paired plates that form the haemal arch. The lateral margin of each lamina is firmly attached to the ventral surface of the caudal vertebral centrum and the medial end fuses to the medial end of the opposite lamina." [AAO:Pugener_2002]
relationship: part_of AAO:0000726 ! haemal_arch

[Term]
id: AAO:0000728
name: nucal_keel
def: "Longitudinal process found in all cervical vertebrae, except the atlas, for the attachment of dorsal head musculature." [AAO:Duellman_and_Trueb_1994]
relationship: part_of AAO:0000709 ! atlas

[Term]
id: AAO:0000729
name: spinal_foramen
def: "Opening on the vertebra for a spinal nerve as it emerges from the spinal canal." [AAO:Francis_1934]
is_a: AAO:0000700 ! vertebral_column_opening

[Term]
id: AAO:0000730
name: foramen_nutritium
def: "Opening on the lateral side of the vertebra for the passage of blood vessels." [AAO:Francis_1934]
is_a: AAO:0000700 ! vertebral_column_opening

[Term]
id: AAO:0000731
name: coccyx
def: "Small, bony element consisting of several fused, rudimentary caudal vertebrae; near metamorphosis the hypochord fuses to the coccyx, thereby forming the urostyle." [AAO:Pugener_2002, AAO:Pugener_and_Maglia_2008]
relationship: part_of AAO:0000734 ! vertebral_column

[Term]
id: AAO:0000732
name: urostyle
def: "Rodlike caudal bony structure unique to anurans that lies within a compartment formed by the elongated, anteriorly oriented pelvic girdle. The urostyle is formed by the fusion of the coccyx and the hypochord." [AAO:Pugener_2002, AAO:Pugener_and_Maglia_2008]
related_synonym: "os coccygei" []
relationship: part_of AAO:0000082 ! caudal_region

[Term]
id: AAO:0000733
name: hypochord
def: "Unsegmented ventral structure in the caudal region of anuran larvae; near metamorphosis the hypochord fuses to the coccyx, thereby forming the urostyle." [AAO:Pugener_2002]
relationship: part_of AAO:0000734 ! vertebral_column

[Term]
id: AAO:0000734
name: vertebral_column
is_a: AAO:0000265 ! larval_structure

[Term]
id: AAO:0000735
name: mid-dorsal_keel
def: "Ridge-shaped structure present on the dorsomedial surface of the neural arch lamina; this structure is produced at the point of junction of the contralateral sides of each neural arch." [AAO:Pugener_2002]
relationship: part_of AAO:0000725 ! neural_arch

[Term]
id: AAO:0000736
name: crista_ventralis
def: "Ridge on the ventral aspect of the humeral shaft that extends from the level of the glenoid head to about one-third to one-half the lenfth of the shaft. It serves for the attachment of the mm pectoralis and supra-coracoideus." [AAO:Francis_1934]
related_synonym: "crista_ventralis_humeri" []
related_synonym: "deltoid crest" []
relationship: part_of AAO:0000679 ! humerus

[Term]
id: AAO:0000737
name: perichordal_tube
def: "Coat around the notochord that originates from cells derived from the sclerotomes." [AAO:Pugener_2002]
relationship: part_of AAO:0000327 ! notochord

[Term]
id: AAO:0000738
name: perichordal_ring
def: "Segmental sections of the perichordal tube that give rise to vertebrae." [AAO:Pugener_2002]
relationship: part_of AAO:0000737 ! perichordal_tube

[Term]
id: AAO:0000739
name: spinous_process
def: "Small, posteriorly directed process at the posterior margin of each neural arch lamina; it is not a neural spine." [AAO:Pugener_2002]
relationship: part_of AAO:0000725 ! neural_arch

[Term]
id: AAO:0000740
name: synsacrum
def: "Complex of synostotically fused vertebrae supporting the pelvic girdle. In anurans, the synsacrum is formed by two vertebrae and the urostyle is fused to its posterior end." [AAO:Pugener_2002]
relationship: part_of AAO:0000724 ! sacral_region

[Term]
id: AAO:0000741
name: uncinate_process
def: "Posteriorly directed process (occasionally directed anteriorly) usually associated with the rib (sometimes with the transverse process) of the third vertebra; they provide the origin of the mm serratus superior, medius, and inferior." [AAO:Pugener_2002]
relationship: part_of AAO:0000545 ! rib

[Term]
id: AAO:0000742
name: epiphysis
def: "Cartilaginous expansion at the distal end of an anterior rib or transverse process that serves for the attachment of muscles suspending the pectoral girdle to the vertebral column." [AAO:Pugener_2002]
relationship: part_of AAO:0000699 ! vertebral_column_skeleton

[Term]
id: AAO:0000743
name: sacral_condyle
def: "Anterior, paired convex facets for articulation with the cotyle(s) of the urostyle." [AAO:LAP]
relationship: part_of AAO:0000552 ! sacrum

[Term]
id: AAO:0000744
name: urostyle_cotyle
def: "Anterior, single or paired concave facets for articulation with the sacral condyle(s)." [AAO:LAP]
related_synonym: "fossa condyloidea ossis coccygei" []
relationship: part_of AAO:0000732 ! urostyle

[Term]
id: AAO:0000745
name: webbing_of_bone
def: "In anurans, pair of bony plates that connect the posteromedial margins of the sacral diapophyses with the lateral margins of the anterior portion of the urostyle." [AAO:Pugener_and_Maglia_2008]
relationship: part_of AAO:0000699 ! vertebral_column_skeleton

[Term]
id: AAO:0000746
name: urostyle_ridge
def: "Longitudinal crest on the dorsal side of the urostyle formed by the caudal neural arches." [AAO:Maglia_et_al_2007]
related_synonym: "crista ossi coccygei" []
relationship: part_of AAO:0000732 ! urostyle

[Term]
id: AAO:0000747
name: appendicular_skeleton
def: "The pectoral and pelvic girdles, which articulate with the axial skeleton, together with their associated limbs, the forelimbs and hind limbs, form the appendicular skeleton." [AAO:Duellman_and_Trueb_1994]
relationship: part_of AAO:0000566 ! skeletal_system

[Term]
id: AAO:0000748
name: suprascapula
def: "Paired, cartilaginous elements located in the dorsolateral shoulder region. Each suprascapula is a flat broad blade that extends medially." [AAO:Maglia_et_al_2007]
related_synonym: "adscapulum" []
related_synonym: "episcapulum" []
related_synonym: "omolita" []
related_synonym: "scapula major" []
relationship: part_of AAO:0000935 ! scapular_area

[Term]
id: AAO:0000749
name: glenoid_fossa
def: "Cavity for the articulation of the forelimb formed by the scapula, coracoid, and clavicle." [AAO:Maglia_et_al_2007]
related_synonym: "glenoid cavity" []
relationship: part_of AAO:0000935 ! scapular_area

[Term]
id: AAO:0000750
name: cleithrum
def: "Paired bones of intramembranous origin. Each cleithrum extends medially from a point near the suprascapular-scapular articulation to invest the anterior margin of the suprascapula, and occasionoally it may extend to the dorsal (medial) surface. Usually, this bone is bifurcate." [AAO:Maglia_et_al_2007]
relationship: part_of AAO:0000935 ! scapular_area

[Term]
id: AAO:0000751
name: scapula
def: "Paired bony elements of endochondral origin. They are situated at the level of the jaw articulation, in a vertical position, with the suprascapular margin being dorsal and the glenoid end being ventral." [AAO:Maglia_et_al_2007]
related_synonym: "collum scapulae" []
related_synonym: "lower shoulder blade" []
related_synonym: "omoplate" []
related_synonym: "scapula minor" []
relationship: part_of AAO:0000935 ! scapular_area

[Term]
id: AAO:0000752
name: pars_acromialis
def: "Prominent structure (anteromedial head) that forms the anterior section of the ventral margin of the scapula." [AAO:Trueb_1973]
relationship: part_of AAO:0000751 ! scapula

[Term]
id: AAO:0000753
name: pars_glenoidalis_of_scapula
def: "Concave structure (posteromedial head) that forms the posterior head of the ventral margin of the scapula. The pars glenoidalis articulates with the humerus, and comprises the dorsal portion of the glenoid fossa." [AAO:Trueb_1973]
relationship: part_of AAO:0000751 ! scapula

[Term]
id: AAO:0000754
name: pectoral_girdle_skeleton
is_a: AAO:0000422 ! pectoral_girdle

[Term]
id: AAO:0000755
name: pectoral_girdle_opening
is_a: AAO:0000422 ! pectoral_girdle

[Term]
id: AAO:0000756
name: crista_dorsalis
def: "Small hooked process on the dorsal aspect of the humeral shaft; it does not extend on to the glenoid head. The m subscapularis is inserted on it." [AAO:Francis_1934]
related_synonym: "crista_dorsalis_humeri" []
relationship: part_of AAO:0000679 ! humerus

[Term]
id: AAO:0000757
name: zonal_area
def: "All those parts of the pectoral girdle ventral and medial to the glenoid fossa." [AAO:Duellman_and_Trueb_1994]
relationship: part_of AAO:0000754 ! pectoral_girdle_skeleton

[Term]
id: AAO:0000758
name: lateral_epicondyle
def: "Rounded projection at the distal head of the humerus (larger and more prominent than the lateral epicondyle) and lateral to the humeral head, which serves as a place of attachment for the mm extensor antebrachii et carpi radialis, extensor digitorum communis, and in part to the m extensor antebrachii et carpi ulnaris." [AAO:Francis_1934, AAO:LAP]
related_synonym: "epicondylus_lateralis_humeri" []
relationship: part_of AAO:0000679 ! humerus

[Term]
id: AAO:0000759
name: omosternum
def: "Proximal portion of the prezonal element of the pectoral girdle. It may be a flat, midventral cartilaginous structure or a calcified or bony element elaborated into a stylum." [AAO:Maglia_et_al_2007]
related_synonym: "episternum" []
related_synonym: "interclavicle" []
related_synonym: "prezonal element" []
related_synonym: "prezonal sternum" []
related_synonym: "sternum superior" []
relationship: part_of AAO:0000937 ! prezonal_element

[Term]
id: AAO:0000760
name: procoracoid
def: "Cartilaginous, paired structures located on the anterolateral portions of the zonal area of the pectoral girdle." [AAO:Maglia_et_al_2007]
related_synonym: "precoracoid" []
relationship: part_of AAO:0000936 ! zonal_element

[Term]
id: AAO:0000761
name: clavicle
def: "Slender, paired bones of intramembranous origin that invest the anterior margins of the procoracoids." [AAO:Maglia_et_al_2007]
related_synonym: "acromial" []
related_synonym: "furcula" []
related_synonym: "os thoracale" []
relationship: part_of AAO:0000936 ! zonal_element

[Term]
id: AAO:0000762
name: epicoracoid
def: "Paired, flat cartilaginous arches that compose the central portion of the zonal area, unites the clavicle and coracoid of each half of the pectoral girdle, and form the medial margins of the pectoral fenestrae." [AAO:Maglia_et_al_2007]
related_synonym: "coracoid cartilage" []
related_synonym: "corpus sterni" []
related_synonym: "entosternal" []
related_synonym: "infracoracoid" []
related_synonym: "sterni ossa media" []
relationship: part_of AAO:0000936 ! zonal_element

[Term]
id: AAO:0000763
name: epicoracoid_bridge
def: "A pair of cartilaginous expansions (one from each epicoracoid cartilage) that project anteriorly. They articulate anteriorly with the omosternum." [AAO:Maglia_et_al_2007]
related_synonym: "procoracoid bridge" []
relationship: part_of AAO:0000762 ! epicoracoid

[Term]
id: AAO:0000764
name: coracoid
def: "Paired cartilaginous structures or endochondral bones located on the posterolateral portions of the zonal area of the pectoral girdle." [AAO:Maglia_et_al_2007]
related_synonym: "clavicula" []
related_synonym: "clavicula posterior" []
related_synonym: "clavicula vera" []
related_synonym: "coracoideum" []
related_synonym: "coracoidien" []
related_synonym: "pars sternalis scapulae" []
relationship: part_of AAO:0000936 ! zonal_element

[Term]
id: AAO:0000765
name: sternum
def: "Single element that constitutes the postzonal area of the pectoral girdle." [AAO:Maglia_et_al_2007]
related_synonym: "cartilaginula quadrata intermedia" []
related_synonym: "hyposternum" []
related_synonym: "sternum inferius" []
relationship: part_of AAO:0000938 ! postzonal_element

[Term]
id: AAO:0000767
name: pelvic_girdle_opening
is_a: AAO:0000426 ! pelvic_girdle

[Term]
id: AAO:0000768
name: pelvic_girdle_skeleton
is_a: AAO:0000426 ! pelvic_girdle

[Term]
id: AAO:0000769
name: pelvic_girdle_symphisis
def: "Medial attachement of the two halves of the pelvic girdle." [AAO:Francis_1934]
relationship: part_of AAO:0000426 ! pelvic_girdle

[Term]
id: AAO:0000770
name: acetabulum
def: "Cavity for the articulation of the proximal bone of the hind limb." [AAO:Maglia_et_al_2007]
related_synonym: "cavite cotyloide" []
relationship: part_of AAO:0000768 ! pelvic_girdle_skeleton

[Term]
id: AAO:0000771
name: acetabular_depression
def: "Central, most concave portion of the acetabulum, which remains open." [AAO:Maglia_et_al_2007]
is_a: AAO:0000767 ! pelvic_girdle_opening

[Term]
id: AAO:0000772
name: ilium
def: "Paired, rodlike endochondral bones that constitute the anterior pelvic girdle." [AAO:Maglia_et_al_2007]
related_synonym: "os ischii" []
relationship: part_of AAO:0000768 ! pelvic_girdle_skeleton

[Term]
id: AAO:0000773
name: ilial_ridge
def: "Longitudinal crest on the dorsal side of the shaft of the ilium." [AAO:Maglia_et_al_2007]
related_synonym: "ala ossis ilei" []
relationship: part_of AAO:0000774 ! ilial_shaft

[Term]
id: AAO:0000774
name: ilial_shaft
def: "Anterior rod that articulates with the sacrum." [AAO:Maglia_et_al_2007]
relationship: part_of AAO:0000772 ! ilium

[Term]
id: AAO:0000775
name: ilial_corpus
def: "Posterior body of the illium that forms the anterior half of the acetabulum." [AAO:Maglia_et_al_2007]
relationship: part_of AAO:0000772 ! ilium

[Term]
id: AAO:0000776
name: glenoid_foramen
def: "Opening on the glenoid fossa." [AAO:LAP]
is_a: AAO:0000755 ! pectoral_girdle_opening

[Term]
id: AAO:0000777
name: epicoracoid_horn
def: "A pair of cartilaginous expansions (one from each epicoracoid cartilage) that project posteriorly. They articulate with the sternum by means of grooves, pouches or fossae in the dorsal surface of the sternum and provide a site for the insertion of a pair of muscles derived from the m. rectus abdominis." [AAO:LAP]
relationship: part_of AAO:0000762 ! epicoracoid

[Term]
id: AAO:0000778
name: supracoracoid_foramen
def: "Opening on the scapulocoracoid bone through which passes the n. supracoracoideus and the corresponding artery and vein." [AAO:Francis_1934]
related_synonym: "foramen supracoracoideum" []
is_a: AAO:0000755 ! pectoral_girdle_opening

[Term]
id: AAO:0000779
name: pectoral_fenestra
def: "Ovoid space on the pectoral girdle limited anteriorly by the procoracoid, medially by the epicoracoid, and posteriorly by the coracoid." [AAO:Maglia_et_al_2007]
related_synonym: "fenestra between procoracoid and coracoid" []
is_a: AAO:0000755 ! pectoral_girdle_opening

[Term]
id: AAO:0000780
name: incisura_coracoidea
def: "Notch that separates the cartilaginous regions of the procoracoid and coracoid." [AAO:Duellman_and_Trueb_1994]
relationship: part_of AAO:0000935 ! scapular_area

[Term]
id: AAO:0000781
name: scapulocoracoid
def: "Fused, ossified portions of the scapula, procoracoid, and coracoid." [AAO:Duellman_and_Trueb_1994]
relationship: part_of AAO:0000935 ! scapular_area

[Term]
id: AAO:0000782
name: medial_epicondyle
def: "Rounded projection at the distal head of the humerus and medial to the humeral head, which serves as a place of attachment for the flexor muscles antogonistic to those that attach to the lateral epicondyle." [AAO:Francis_1934, AAO:LAP]
related_synonym: "epicondylus_medialis_humeri" []
relationship: part_of AAO:0000679 ! humerus

[Term]
id: AAO:0000783
name: fovea_capitis
def: "Ovoid roughened pit, which is situated a little below and behind the center of the head, and serves as a site of attachment for ligaments." [AAO:LAP]
relationship: part_of AAO:0000679 ! humerus

[Term]
id: AAO:0000784
name: ulnar_condyle
def: "Semi-elliptical ball located at the lower end of the humerus, adjacent to the humeral ball." [AAO:Francis_1934]
relationship: part_of AAO:0000679 ! humerus

[Term]
id: AAO:0000785
name: trochlear_groove_of_humerus
def: "Furrow between the humeral head and the ulnar condyle." [AAO:Francis_1934]
relationship: part_of AAO:0000679 ! humerus

[Term]
id: AAO:0000786
name: fossa_cubitalis_ventralis
def: "Depresion on the distal end of the humerus, just anterior to the humeral head, in which the end of the radius fits when the forelimb is flexed." [AAO:Francis_1934, LAP:Maglia_et_al_2007]
relationship: part_of AAO:0000679 ! humerus

[Term]
id: AAO:0000787
name: collum_antibrachii
def: "In a fused radio-ulna, the proximal portion of the compound bone (where the sulcus longitudinalis is barely evident or absent) is a cylindrical pillar." [AAO:LAP]
relationship: part_of AAO:0000200 ! fore_epipodium

[Term]
id: AAO:0000788
name: radius
def: "One of the two long bones of endochondral origin of the fore-epipodium; it is located on the lateral side of the ulna. Its upper end articulates with both the humerus and the ulna, whereas the lower articulates with the carpals." [AAO:LAP]
relationship: part_of AAO:0000200 ! fore_epipodium

[Term]
id: AAO:0000789
name: ulna
def: "One of the two long bones of endochondral origin of the fore-epipodium; it is located on the medial (inner) side of the radius. The upper end of the ulna articulates with the lower end of the humerus forming a strong hinge joint with the carpals, whereas the lower articulates with the carpals." [AAO:LAP]
relationship: part_of AAO:0000200 ! fore_epipodium

[Term]
id: AAO:0000790
name: radiale
def: "One of two element that constitute the basal row of carpals. It articulates proximally with the radius, mesially with the ulnare (or pars intermedia of the ulnare when the ulnare is fused to the intermedium) and distally with the centrale (also recognized by some authors as element Y). This element originates from one or two condensation centers. Occasionally it may fuse to carpal 5(4), the ulnare, or other elements." [AAO:Fabrezi_1992, AAO:Fabrezi_and_Alberch_1996, AAO:Francis_1934]
relationship: part_of AAO:0000201 ! fore_mesopodium

[Term]
id: AAO:0000791
name: episternum
def: "Distal, flat, cartilaginous element of the prezonal element of the pectoral girdle." [AAO:LAP]
relationship: part_of AAO:0000937 ! prezonal_element

[Term]
id: AAO:0000792
name: anterior_ramus_of cleithrum
def: "Subdivision of the cleithrum that extends along the anterior edge of the suprascapula." [AAO:Trueb_1973]
relationship: part_of AAO:0000750 ! cleithrum

[Term]
id: AAO:0000793
name: anomocoelous
def: "Stegochordal slightly biconcave or flat terminally vertebral centrum. Each intervertebral cartilage is subdivided anteriorly and posteriorly, producing a free intervertebral element between adjacent vertebrae. This element subsequently ossifies and remains free." [AAO:Trueb_1973]
is_a: AAO:0000697 ! centrum

[Term]
id: AAO:0000794
name: displasiocoelous
def: "Vertebral column in which the first seven vertebrae have holochordal centra and the intervertebral cartilages are posteriorly subdivided in the procoelous manner. The eighth presacral vertebra has a holochordal centrum and the intervertebral cartilage is subdivided in the opisthocoelous manner. Thus, the first seven presacral vertebrae are concave anteriorly and convex posteriorly, whereas the eighth is biconcave." [AAO:Trueb_1973]
is_a: AAO:0000697 ! centrum

[Term]
id: AAO:0000795
name: intervertebral_cartilage
def: "Block of cartilage, which usually ossifies, that lies between successive vertebral centra." [AAO:Trueb_1973]
relationship: part_of AAO:0000691 ! vertebra

[Term]
id: AAO:0000796
name: imbricate_neural_arch
def: "Overlapping neural arches that obscure the spinal cord dorsally." [AAO:Trueb_1973]
is_a: AAO:0000725 ! neural_arch

[Term]
id: AAO:0000797
name: non-imbricate_neural_arch
def: "Neural arches that do not overlap, thus exposing the spinal cord dorsally." [AAO:Trueb_1973]
is_a: AAO:0000725 ! neural_arch

[Term]
id: AAO:0000798
name: presacral_shield
def: "Dorsal, dermal plate of bone that overlies the presacral vertebrae. Such shield usually has irregular, sculptured surfaces, frequently is broadly expanded, and may be composed of several separate plates." [AAO:Trueb_1973]
relationship: part_of AAO:0000612 ! trunk_region

[Term]
id: AAO:0000799
name: cartilago_paraglenoidalis
def: "Strip of cartilage that separates the coracoid from the scapula." [AAO:Stephenson_1952]
relationship: part_of AAO:0000935 ! scapular_area

[Term]
id: AAO:0000800
name: intercotylar_space
def: "Space between the atlantal cotyles." [AAO:LAP]
related_synonym: "spatium interglenoidale" []
relationship: part_of AAO:0000709 ! atlas

[Term]
id: AAO:0000801
name: caput_glenoidale
def: "Convex articular facet of the vertebral centrum for the articulation with the adjacent centrum." [AAO:LAP]
relationship: part_of AAO:0000697 ! centrum

[Term]
id: AAO:0000802
name: fossa_glenoidalis
def: "Concave articular facet of the vertebral centrum for the articulation with the adjacent centrum." [AAO:LAP]
relationship: part_of AAO:0000697 ! centrum

[Term]
id: AAO:0000803
name: sulcus_articularis_lateralis
def: "In a zygapophysis that has ridges and sulci, the lateral canal between the carina distalis and the carina medialis." [AAO:LAP]
relationship: part_of AAO:0000710 ! zygapophysis

[Term]
id: AAO:0000804
name: sulcus_articularis_medialis
def: "In a zygapophysis that has ridges and sulci, the medial canal between the carina medialis and the carina proximalis." [AAO:LAP]
relationship: part_of AAO:0000710 ! zygapophysis

[Term]
id: AAO:0000805
name: carina_proximalis
def: "In a zygapophysis that has ridges and sulci, the proximal ridge." [AAO:LAP]
relationship: part_of AAO:0000710 ! zygapophysis

[Term]
id: AAO:0000806
name: carina_medialis
def: "In a zygapophysis that has ridges and sulci, the medial ridge." [AAO:LAP]
relationship: part_of AAO:0000710 ! zygapophysis

[Term]
id: AAO:0000807
name: carina_distalis
def: "In a zygapophysis that has ridges and sulci, the distal ridge." [AAO:LAP]
relationship: part_of AAO:0000710 ! zygapophysis

[Term]
id: AAO:0000808
name: parasagittal_processes
def: "Paired, posteriorly directed process at the posterior margin of each neural arch lamina." [AAO:Cannatella_1985]
relationship: part_of AAO:0000725 ! neural_arch

[Term]
id: AAO:0000809
name: accessory_articulation
def: "Paired, additional vertebral articulations located medial to the intervertebral space, adjacent to the vertebral centrum." [AAO:Cannatella_1985]
relationship: part_of AAO:0000691 ! vertebra

[Term]
id: AAO:0000810
name: fissura_sagittalis
def: "Medial groove in the longitudinal ridge of the urostyle formed by the incomplete dorsal fusion of the caudal neural arches." [AAO:Maglia_et_al_2007]
relationship: part_of AAO:0000746 ! urostyle_ridge

[Term]
id: AAO:0000811
name: glenoid_end_of_clavicle
def: "Lateral end of the clavicle, which usually lies in close proximity to the pars acromialis of the scapula, and occassionally may fuse to it." [AAO:Cannatella_1985]
related_synonym: "extremitas glenoidalis" []
relationship: part_of AAO:0000761 ! clavicle

[Term]
id: AAO:0000812
name: sternal_end_of_clavicle
def: "Medial end of the clavicle, which usually lies on the ventral side of the epicoracoid cartilage, just posterior to the epicoracoid bridge." [AAO:Maglia_et_al_2007]
related_synonym: "extremitas medialis" []
related_synonym: "medial end" []
relationship: part_of AAO:0000761 ! clavicle

[Term]
id: AAO:0000813
name: sulcus_pro_cartilagine_praecoracoidealis
def: "Canal on the posterior aspect of the clavicle that accomodates the anterior margin of the procoracoid cartilage." [AAO:LAP]
relationship: part_of AAO:0000761 ! clavicle

[Term]
id: AAO:0000814
name: glenoid_head_of_coracoid
def: "Lateral end of the coracoid, which forms the medial portion of the glenoid fossa." [AAO:Maglia_et_al_2007]
related_synonym: "intumescentia_glenoidalis" []
relationship: part_of AAO:0000764 ! coracoid

[Term]
id: AAO:0000815
name: sternal_head_of_coracoid
def: "Medial end of the coracoid, which is synchondrotically fused to the epicoracoid cartilage." [AAO:Maglia_et_al_2007]
related_synonym: "pars epicoracoidealis" []
relationship: part_of AAO:0000764 ! coracoid

[Term]
id: AAO:0000816
name: margo_fenestralis
def: "Anterior margin of the coracoid, which forms the posterior edge of the pectoral fenestra." [AAO:LAP]
relationship: part_of AAO:0000764 ! coracoid

[Term]
id: AAO:0000817
name: margo_posterior
def: "Posterior margin of the coracoid." [AAO:LAP]
relationship: part_of AAO:0000764 ! coracoid

[Term]
id: AAO:0000818
name: margo_anterior_of_scapula
def: "Anterior margin of the scapula." [AAO:LAP]
relationship: part_of AAO:0000751 ! scapula

[Term]
id: AAO:0000819
name: margo_clavicularis
def: "Inferior margin of the pars acromialis of the scapula, which articulates with the clavicule." [AAO:LAP]
relationship: part_of AAO:0000751 ! scapula

[Term]
id: AAO:0000820
name: margo_posterior_of_scapula
def: "Posterior margin of the scapula." [AAO:LAP]
relationship: part_of AAO:0000751 ! scapula

[Term]
id: AAO:0000821
name: margo_suprascapularis
def: "Superior margin of the scapula, which articulates with the suprascapula." [AAO:LAP]
relationship: part_of AAO:0000751 ! scapula

[Term]
id: AAO:0000822
name: pars_suprascapularis
def: "Superior portion of the scapula, which is thinner than the rest of the shaft." [AAO:LAP]
relationship: part_of AAO:0000751 ! scapula

[Term]
id: AAO:0000823
name: sinus_interglenoidalis
def: "Notch or indentation between the pars glenoidalis and pars acromialis of the scapula." [AAO:LAP]
relationship: part_of AAO:0000751 ! scapula

[Term]
id: AAO:0000824
name: tenuitas_cristaeformis
def: "Leading (anterior) portion of the scapula, which is thinner than the rest of the shaft." [AAO:LAP]
relationship: part_of AAO:0000751 ! scapula

[Term]
id: AAO:0000825
name: crista_longitudinalis
def: "Longitudinal ridge on the medial (inner) face of the scapula." [AAO:LAP]
relationship: part_of AAO:0000751 ! scapula

[Term]
id: AAO:0000826
name: acromion
def: "Anterior rounded projection of the pars acromialis of the scapula." [AAO:LAP]
relationship: part_of AAO:0000752 ! pars_acromialis

[Term]
id: AAO:0000827
name: margo_anterior_of_cleithrum
def: "Anterior margin of the anterior ramus of the cleithrum." [AAO:LAP]
relationship: part_of AAO:0000750 ! cleithrum

[Term]
id: AAO:0000828
name: margo_posterior_of_cleithrum
def: "Posterior margin of the posterior ramus of the cleithrum." [AAO:LAP]
relationship: part_of AAO:0000750 ! cleithrum

[Term]
id: AAO:0000829
name: margo_scapularis
def: "Lateral margin of the suprascapula, which articulates with the scapula." [AAO:LAP]
relationship: part_of AAO:0000750 ! cleithrum

[Term]
id: AAO:0000830
name: margo_vertebralis
def: "Medial margin of the suprascapula, which lies dorsal to the vertebral column." [AAO:LAP]
relationship: part_of AAO:0000750 ! cleithrum

[Term]
id: AAO:0000831
name: spina_acromioidea
def: "Small process of the lamina recurvata that extends laterally toward the scapular-suprascapular articulation." [AAO:LAP]
relationship: part_of AAO:0000750 ! cleithrum

[Term]
id: AAO:0000832
name: anterior_lamina_recurvata
def: "Portion of the anterior ramus of the cleithrum that invest the anterior margin of the suprascapula, extending onto its dorsal surface." [AAO:LAP]
relationship: part_of AAO:0000750 ! cleithrum

[Term]
id: AAO:0000833
name: sinus_dorsalis
def: "Notch or indentation between the anterior and posterior rami of the cleithrum." [AAO:LAP]
relationship: part_of AAO:0000750 ! cleithrum

[Term]
id: AAO:0000834
name: posterior_lamina_recurvata
def: "Portion of the posterior ramus of the cleithrum that invests the posterior margin of the suprascapula, extending onto its dorsal surface." [AAO:LAP]
relationship: part_of AAO:0000750 ! cleithrum

[Term]
id: AAO:0000835
name: glenoid_head
def: "Hemispherical ball on the proximal end of the humerus that fits into the glenoid cavity of the pectoral girdle to form the shoulder joint." [AAO:Maglia_et_al_2007]
related_synonym: "caput humeri" []
relationship: part_of AAO:0000679 ! humerus

[Term]
id: AAO:0000836
name: crista_lateralis
def: "Ridge on the lateral aspect of the humeral shaft located just anterior to the radial (lateral) epicondyle." [AAO:LAP]
relationship: part_of AAO:0000679 ! humerus

[Term]
id: AAO:0000837
name: crista_medialis
def: "Ridge on the medial aspect of the humeral shaft that extends from the level of the middle portion of the shaft to ulnar (medial) epicondyle." [AAO:LAP]
relationship: part_of AAO:0000679 ! humerus

[Term]
id: AAO:0000838
name: humeral_head
def: "Hemispherical ball located at the lower end of the humerus that stands out prominently from the surrounding structures toward the flexor surface of the forelimb and fits into the socket joint of the olecranon process." [AAO:Francis_1934]
related_synonym: "eminentia capitata" []
related_synonym: "radial condyle" []
relationship: part_of AAO:0000679 ! humerus

[Term]
id: AAO:0000839
name: crista_radii
def: "Small ridge on the lateral aspect of the radial shaft, located at the level of the collum antibrachii." [AAO:LAP]
relationship: part_of AAO:0000788 ! radius

[Term]
id: AAO:0000840
name: capitulum_of_radius
def: "Lateral portion of the proximal (upper) articular surface of the radius that consists of an eminence with a rounded apex." [AAO:LAP]
relationship: part_of AAO:0000788 ! radius

[Term]
id: AAO:0000841
name: capitulum_radii
def: "Small eminence on the distal articular head of the radius." [AAO:LAP]
relationship: part_of AAO:0000788 ! radius

[Term]
id: AAO:0000842
name: capitulum_ulnae
def: "Small eminence on the distal articular head of the ulna." [AAO:LAP]
relationship: part_of AAO:0000789 ! ulna

[Term]
id: AAO:0000843
name: olecranon
def: "Large and thick process situated at the proximal (upper) end of the ulna. Its inner face forms the medial articular surface that articulates with the humeral head." [AAO:LAP]
related_synonym: "ulnar_process" []
relationship: part_of AAO:0000789 ! ulna

[Term]
id: AAO:0000844
name: sulcus_longitudinalis
def: "In a fused radio-ulna, longitudinal furrow that demarcates the area of fusion of both elements. This sulcus is deep in the distal portion of the compound bone, but barely evident or absent at the proximal end." [AAO:Maglia_et_al_2007]
relationship: part_of AAO:0000901 ! radio-ulna

[Term]
id: AAO:0000845
name: ulnare
def: "One of two element that constitute the basal row of carpals. It articulates with the ulna, radius, radiale, centrale (element Y), and carpal 5(4). This element originates from one condensation center or the fusion of two elements (ulnare and intermedium). Occasionally it may fuse to carpal 5(4), the radiale, or other elements." [AAO:Fabrezi_1992, AAO:Fabrezi_and_Alberch_1996, AAO:Francis_1994]
relationship: part_of AAO:0000201 ! fore_mesopodium

[Term]
id: AAO:0000846
name: element_Y_of_fore_mesopodium
def: "Oval carpal element that is located on the anteromedial side of the radiale and the anterolateral side of the ulnare. Anteriorly, it articulates with carpals 1 through 4 (or 2 through 5 according to some authors). It is also recognized as centrale by some authors. This element originates from one, two, or three condensation centers. Occasionally it may fuse to carpal 2(1), carpal 3(2), the ulnare, or other elements." [AAO:Fabrezi_1992, AAO:Fabrezi_and_Alberch_1996, AAO:Francis_1934]
relationship: part_of AAO:0000201 ! fore_mesopodium

[Term]
id: AAO:0000847
name: distal_carpal
def: "Series of elements that articulate with the metacarpals." [AAO:Francis_1934]
related_synonym: "basale" []
relationship: part_of AAO:0000201 ! fore_mesopodium

[Term]
id: AAO:0000848
name: carpal_2(1)
def: "Small element that articulates with the prepollex, metacarpal II(I) and metacarpal III(II). It may be fused to element Y or carpal 3(2)." [AAO:Fabrezi_1992, AAO:LAP]
is_a: AAO:0000847 ! distal_carpal

[Term]
id: AAO:0000849
name: carpal_3(2)
def: "Small element that articulates anteriorly with metacarpal III(II). It may be fused to carpals 2(1), 4(3), 5(4), or other elements." [AAO:Fabrezi_1992, AAO:LAP]
is_a: AAO:0000847 ! distal_carpal

[Term]
id: AAO:0000850
name: carpal_4(3)
def: "Small element that articulates anteriorly with metacarpal IV(III). It may be fused to carpal 3(2), 5(4), or other elements." [AAO:Fabrezi_1992, AAO:LAP]
is_a: AAO:0000847 ! distal_carpal

[Term]
id: AAO:0000851
name: carpal_5(4)
def: "Small element that articulates anteriorly with metacarpal IV(V). It may be fused to carpal 4(3), 5(4), the ulnare, radiale, or other elements." [AAO:Fabrezi_1992, AAO:LAP]
is_a: AAO:0000847 ! distal_carpal

[Term]
id: AAO:0000852
name: prepollex
def: "Two or more elements located ventral and medial to the metacarpal of digit II(I). The proximal prepollex is small and round whereas distal prepollex 1 is usually large and wedge-shaped. When more elements are present, they are smaller than previous elements." [AAO:Fabrezi_and_Alberch_1996, AAO:Maglia_et_al_2007]
related_synonym: "cartilago_pre-pollicis" []
relationship: part_of AAO:0000201 ! fore_mesopodium

[Term]
id: AAO:0000853
name: metacarpal_II(I)
def: "Dumb-bell-shaped bone of endochondral origin with cartilaginous epiphyses that articulates with the prepollex and carpal 2(1) or carpal 2+3(1+2) proximally and with the proximal phalanx of digit II(I) distally." [AAO:Fabrezi_1992, AAO:Maglia_et_al_2007]
is_a: AAO:0000946 ! fore_metapodium

[Term]
id: AAO:0000854
name: metacarpal_III(II)
def: "Dumb-bell-shaped bone of endochondral origin with cartilaginous epiphyses that articulates with carpal 3(2) proximally and with the proximal phalanx of digit III(II) distally." [AAO:Fabrezi_1992, AAO:Maglia_et_al_2007]
is_a: AAO:0000946 ! fore_metapodium

[Term]
id: AAO:0000855
name: metacarpal_V(IV)
def: "Dumb-bell shaped bones of endochondral origin with cartilaginous epiphyses that articulates with carpal 5(4) proximally and with the proximal phalanx of digit V(IV) distally." [AAO:Fabrezi_1992, AAO:Maglia_et_al_2007]
is_a: AAO:0000946 ! fore_metapodium

[Term]
id: AAO:0000856
name: intercalary_element_of_fore_digit
def: "Small elements of endochondral origin present in all digits of the manus. Each intercalary element articulates with the anteroventral end of the penultimate phalanx proximally and the distal phalanx distally." [AAO:Maglia_et_al_2007]
relationship: part_of AAO:0000857 ! fore_digit

[Term]
id: AAO:0000857
name: fore_digit
def: "One of the fingers of the manus." [AAO:LAP]
relationship: part_of AAO:0000202 ! forelimb_skeleton

[Term]
id: AAO:0000858
name: forelimb_opening
is_a: AAO:0000205 ! forelimb

[Term]
id: AAO:0000859
name: foramen_perforans_carpi
def: "Opening for the passage of the perforans carpi artery from the ventral to the dorsal side. It perforates the compound ulnare + intermedium." [AAO:Francis_1934]
is_a: AAO:0000856 ! intercalary_element_of_fore_digit

[Term]
id: AAO:0000860
name: ischium
def: "Paired bones of endochondral origin that constitute the posterior elements of the pelvic girdle. They are synostotically fused to each other and form the posterior part of the acetabulum." [AAO:Duellman_and_Trueb_1994, AAO:Maglia_et_al_2007]
relationship: part_of AAO:0000768 ! pelvic_girdle_skeleton

[Term]
id: AAO:0000861
name: pubis
def: "Paired, cartilaginous (ocassionally calcified) elements that form the ventral portion of the pelvic girdle. Each is located ventral to the acetabulum between the anteroventral margin of the ischium and the posteroventral margin of the illium. When the element calcifies or ossifies, its articulation with adjacent elements is difficult to distinguish. Both pubes are synchondrotically fused to one another." [AAO:Duellman_and_Trueb_1994, AAO:Maglia_et_al_2007]
related_synonym: "cartilago remanens" []
relationship: part_of AAO:0000768 ! pelvic_girdle_skeleton

[Term]
id: AAO:0000862
name: pubo-ischium
def: "Composite element formed by the fusion of the ischium and pubis." [AAO:Francis_1943]
related_synonym: "ilio-pubis" []
relationship: part_of AAO:0000768 ! pelvic_girdle_skeleton

[Term]
id: AAO:0000863
name: obturator_foramen
def: "Small opening for the passage of the obturatorius nerve that perforates the pubis." [AAO:Francis_1934]
is_a: AAO:0000767 ! pelvic_girdle_opening

[Term]
id: AAO:0000864
name: acetabular_rim
def: "Cartilaginous ring that forms the entire acetabular margin." [AAO:Maglia_et_al_2007]
relationship: part_of AAO:0000770 ! acetabulum

[Term]
id: AAO:0000865
name: epileon
def: "Dorsal extremity of the ilial shaft, which remains cartilaginous." [AAO:Francis_1934]
relationship: part_of AAO:0000774 ! ilial_shaft

[Term]
id: AAO:0000866
name: agger_limitans_anterior
def: "Shelf-like expansion of the ilial corpus that forms the anterior border of the acetabulum." [AAO:Maglia_et_al_2007]
relationship: part_of AAO:0000775 ! ilial_corpus

[Term]
id: AAO:0000867
name: agger_limitans_posterior
def: "Shelf-like expansion of the ischium that forms the posterior border of the acetabulum." [AAO:Maglia_et_al_2007]
relationship: part_of AAO:0000860 ! ischium

[Term]
id: AAO:0000868
name: supra-acetabular_expansion
def: "Dorsal portion of the ilial corpus, located above the acetabulum." [AAO:Maglia_et_al_2007]
related_synonym: "dorsal acetabular expansion" []
related_synonym: "pars ascendens ilei" []
relationship: part_of AAO:0000775 ! ilial_corpus

[Term]
id: AAO:0000869
name: ilial_protuberance
def: "Small, dorsolaterally projecting knob located just anterior to the supra-acetabular expansion and about the level of the anterior border of the acetabulum." [AAO:Maglia_et_al_2007]
related_synonym: "dorsal protuberance" []
related_synonym: "tuber_superior" []
relationship: part_of AAO:0000774 ! ilial_shaft

[Term]
id: AAO:0000870
name: preacetabular_expansion
def: "Ventral portion of the ilial corpus, located anteroventral to the acetabulum." [AAO:Maglia_et_al_2007]
related_synonym: "pars descendens ilei" []
related_synonym: "ventral acetabular expansion" []
relationship: part_of AAO:0000775 ! ilial_corpus

[Term]
id: AAO:0000871
name: fossula_tuberis_superioris
def: "Small depression dorsal to the proximal portion of the collum ilei and ventral to the ilial protuberance." [AAO:LAP]
relationship: part_of AAO:0000775 ! ilial_corpus

[Term]
id: AAO:0000872
name: collum_ilei
def: "Cyllindrical pillar that originates anterior to the acetabulum and extends to the ilial shaft." [AAO:LAP]
relationship: part_of AAO:0000775 ! ilial_corpus

[Term]
id: AAO:0000873
name: pars_cylindriformis_ilei
def: "Elongate, cylindrical structure on the ventral side of the shaft of the ilium that extends through its entire length." [AAO:LAP]
relationship: part_of AAO:0000774 ! ilial_shaft

[Term]
id: AAO:0000874
name: crista_ischii
def: "Crest on the posterior side of the ischium, which may also extend to the posteroventral aspect of pubis." [AAO:LAP]
relationship: part_of AAO:0000860 ! ischium

[Term]
id: AAO:0000875
name: spina_pelvis_posterior
def: "Small, rounded process on the anterodorsal margin of the ischium, just posterior to the area of articulation with the ilium." [AAO:LAP]
relationship: part_of AAO:0000860 ! ischium

[Term]
id: AAO:0000876
name: spina_pelvis_anterior
def: "Small, rounded process on the anteroventral margin of the preacetabular expansion of the ilial corpus." [AAO:LAP]
relationship: part_of AAO:0000775 ! ilial_corpus

[Term]
id: AAO:0000877
name: intumescentia_bilateralis_inferior
def: "Small protuberance on the ischium, located close to its posteroventral margin." [AAO:LAP]
relationship: part_of AAO:0000860 ! ischium

[Term]
id: AAO:0000878
name: intumescentia_bilateralis_superior
def: "Small protuberance on the ischium, located at the level of the superior margin of the acetabulum and close to its posterior margin." [AAO:LAP]
relationship: part_of AAO:0000860 ! ischium

[Term]
id: AAO:0000879
name: incisura_terminalis
def: "Small indentation on the posterior margin of the ischium, ventral to the intumescentia bilateralis superior." [AAO:LAP]
relationship: part_of AAO:0000860 ! ischium

[Term]
id: AAO:0000880
name: crista_hypertrophica
def: "Large protuberance on the dorsal aspect of the ischium that extends from the ischio-ilium articulation to the spina pelvis posterior." [AAO:LAP]
relationship: part_of AAO:0000860 ! ischium

[Term]
id: AAO:0000881
name: lamina_terminalis
def: "In those cases in which the interilial region is broadly expanded and the pubis is extremely reduced, the anterior margin of the ischium forms an expanded area." [AAO:LAP]
relationship: part_of AAO:0000860 ! ischium

[Term]
id: AAO:0000882
name: interilial_region
def: "Area of convergence of the ilial shafts. When the preacetabular ilium is narrow, the interilial configuration is V-shaped or narrowly rounded, whereas when the interilial region is broadly expanded the interilial configuration is U-shaped." [AAO:Baez_and_Trueb_1997]
relationship: part_of AAO:0000772 ! ilium

[Term]
id: AAO:0000883
name: recessus_coccygealis
def: "Area dorsal to the pelvic girdle symphysis, between the dorsal portions of the ilial corpora, where lies the posterior terminus of the urostyle." [AAO:Maglia_et_al_2007]
relationship: part_of AAO:0000774 ! ilial_shaft

[Term]
id: AAO:0000884
name: epipubis
def: "Small prepubic element formed by a plate of cartilage (which may calcify in the adult) that is synchondrotically united with the pubis." [AAO:Duellman_and_Trueb_1994]
relationship: part_of AAO:0000768 ! pelvic_girdle_skeleton

[Term]
id: AAO:0000885
name: postpubis
def: "Paired cartilaginous rods that lie within the copulatory organ (or so-called tail) and are attached to the posteroventral part of the pelvic girdle." [AAO:Duellman_and_Trueb_1994]
related_synonym: "Nobelian bone" []
relationship: part_of AAO:0000768 ! pelvic_girdle_skeleton

[Term]
id: AAO:0000886
name: ypsiloid_cartilage
def: "Y-shaped cartilage lying in the middle line, anterior to the pubo-ischium with which it articulates. It lies dorsal to the rectus abdominis muscle with which it articulates." [AAO:Francis_1934]
related_synonym: "abdominal sternum" []
related_synonym: "Cartilago epipubes" []
related_synonym: "cartilago marsupial" []
related_synonym: "cartilago ypsiloidea" []
related_synonym: "cartilago ypsiloides" []
relationship: part_of AAO:0000768 ! pelvic_girdle_skeleton

[Term]
id: AAO:0000887
name: hind_propodium
def: "Segment of the hindleg corresponding to the humerus." [AAO:Duellman_and_Trueb_1994]
is_a: AAO:0000217 ! hind_limb_skeleton

[Term]
id: AAO:0000888
name: hind_digit
def: "One of the toes of the pes." [AAO:LAP]
relationship: part_of AAO:0000217 ! hind_limb_skeleton

[Term]
id: AAO:0000889
name: femur
def: "Paired, elongate, cylindrical bones of endochondral origin that form the thighs, extending from the pelvic girdles to the knees." [AAO:Maglia_et_al_2007]
relationship: part_of AAO:0000887 ! hind_propodium

[Term]
id: AAO:0000890
name: tibia
def: "One of the two long bones of endochondral origin of the hind-epipodium; it is a straight, simple bone whose section is more or less rectangular at the ends and circular at its central portion." [AAO:Francis_1934]
relationship: part_of AAO:0000216 ! hind_epipodium

[Term]
id: AAO:0000891
name: fibula
def: "One of the two long bones of endochondral origin of the hind-epipodium; it is a rather more slender bone than the tibia but of about the same length." [AAO:Francis_1934]
relationship: part_of AAO:0000216 ! hind_epipodium

[Term]
id: AAO:0000892
name: acetabular_head
def: "Proximal head of the femur, which articulates with the acetabulum." [AAO:Maglia_et_al_2007]
related_synonym: "caput femoris" []
relationship: part_of AAO:0000889 ! femur

[Term]
id: AAO:0000893
name: distal_head
def: "Head of the femur that articulates with the tibia and fibula." [AAO:Maglia_et_al_2007]
relationship: part_of AAO:0000889 ! femur

[Term]
id: AAO:0000894
name: femoral_ridge
def: "Low crest that arises just behind the acetabular head and extends distally for about one-third the length of the femoral shaft." [AAO:Maglia_et_al_2007]
related_synonym: "crista femoris" []
relationship: part_of AAO:0000889 ! femur

[Term]
id: AAO:0000895
name: trochlear_groove_of_femur
def: "Canal on the posteroventral surface of the acetabular head, which articulates with the ischial process on the rim of the acetabulum." [AAO:Francis_1934]
relationship: part_of AAO:0000892 ! acetabular_head

[Term]
id: AAO:0000896
name: foveal_depression
def: "Ovoid roughened pit situated on the dorsal and anteroventral surface of the acetabular head wherein the ligaments attaching the bone to the acetabulum are inserted." [AAO:Francis_1934]
relationship: part_of AAO:0000892 ! acetabular_head

[Term]
id: AAO:0000897
name: femoral_trochanter
def: "Process on the ventral surface of the shaft of the femur." [AAO:Francis_1934]
relationship: part_of AAO:0000889 ! femur

[Term]
id: AAO:0000898
name: trochanteric_crest
def: "Paired ridges on the ventral surface of the femoral shaft that run toward the femoral trochanter; the posterior crest is less developed." [AAO:Francis_1934]
relationship: part_of AAO:0000889 ! femur

[Term]
id: AAO:0000899
name: tibial_condyle
def: "Convex articular facet of the distal head of the femur that articulates with the proximal head of the tibia." [AAO:Francis_1934]
relationship: part_of AAO:0000893 ! distal_head

[Term]
id: AAO:0000900
name: fibular_condyle
def: "Convex articular facet of the distal head of the femur that articulates with the proximal head of the fibula." [AAO:LAP]
relationship: part_of AAO:0000893 ! distal_head

[Term]
id: AAO:0000901
name: radio-ulna
def: "Paired, long bones of endochondral origin formed by the fusion of the radius and ulna." [AAO:Maglia_et_al_2007]
relationship: part_of AAO:0000200 ! fore_epipodium

[Term]
id: AAO:0000902
name: tibiofibula
def: "Paired, endochondral bones formed by the fusion of the tibia and fibula. They form the shanks, extending from the knees to the ankles." [AAO:Maglia_et_al_2007]
related_synonym: "os cruris" []
relationship: part_of AAO:0000216 ! hind_epipodium

[Term]
id: AAO:0000903
name: tibial_crest
def: "Ridge that arises from the dorso-masial side of the extensor surface of the tibia. It receives the insertion of the tendon of the extensor ilio-tibialis muscle." [AAO:Francis_1934]
relationship: part_of AAO:0000890 ! tibia

[Term]
id: AAO:0000904
name: apophysis_distalis_of_tibiofibula
def: "Swelling on the extensor surface of the distal head of the tibiofibula." [AAO:LAP]
relationship: part_of AAO:0000902 ! tibiofibula

[Term]
id: AAO:0000905
name: caput_ossis_cruris
def: "Proximal head of the tibiofibula that articulates with the distal head of the femur." [AAO:LAP]
relationship: part_of AAO:0000902 ! tibiofibula

[Term]
id: AAO:0000906
name: sulcus_pro_musculo_extensori_cruris_brevis
def: "Small canal on the proximal head of to the tibiofibula, lateral to the apophysis distalis, for the insertion of the cruris brevis muscle." [AAO:LAP]
relationship: part_of AAO:0000902 ! tibiofibula

[Term]
id: AAO:0000907
name: eminentia_arcuata
def: "Small crest on the extensor surface of the proximal head of the tibiofibula (tibial side)." [AAO:LAP]
relationship: part_of AAO:0000902 ! tibiofibula

[Term]
id: AAO:0000908
name: sulcus_distalis_ossis_cruris
def: "In a fused tibiofibula, longitudinal furrow in the distal portion of the compound bone that demarcates the area of fusion of both elements." [AAO:LAP]
relationship: part_of AAO:0000902 ! tibiofibula

[Term]
id: AAO:0000909
name: sulcus_proximalis_ossis_cruris
def: "In a fused tibiofibula, longitudinal furrow in the proximal portion of the compound bone that demarcates the area of fusion of both elements." [AAO:LAP]
relationship: part_of AAO:0000902 ! tibiofibula

[Term]
id: AAO:0000910
name: hind_limb_opening
is_a: AAO:0000219 ! hind_limb

[Term]
id: AAO:0000911
name: foramen_nutritium_exterius
def: "Foramen for the tibial artery and vein and the deep peroneal nerve; it pierces through the midpoint of the shaft of the tibiofibula." [AAO:Maglia_et_al_2007]
is_a: AAO:0000910 ! hind_limb_opening

[Term]
id: AAO:0000912
name: tibiale
def: "One of two element that constitute the basal row of tarsals. The tibiale constitutes the postaxial element. In salamanders this element is aproximatelly rounded, whereas in anurans it is an elongate, cylindrical bone with the proximal and distal heads fused to the heads of the fibulare." [AAO:LAP]
related_synonym: "calcaneus" []
relationship: part_of AAO:0000220 ! hind_mesopodium

[Term]
id: AAO:0000913
name: fibulare
def: "One of two element that constitute the basal row of tarsals. The fibulare constitutes the preaxial element. In salamanders this element is aproximatelly rounded, whereas in anurans it is an elongate, cylindrical bone with the proximal and distal heads fused to the heads of the tibiale." [AAO:Maglia_et_al_2007]
related_synonym: "astragalus" []
relationship: part_of AAO:0000220 ! hind_mesopodium

[Term]
id: AAO:0000914
name: distal_tarsal
def: "Series of elements that articulate with the metatarsals." [AAO:LAP]
relationship: part_of AAO:0000220 ! hind_mesopodium

[Term]
id: AAO:0000915
name: spatium_intertarsale
def: "Separation of the tibiale and fibulare along their longitudinal axia." [AAO:Maglia_et_al_2007]
is_a: AAO:0000910 ! hind_limb_opening

[Term]
id: AAO:0000916
name: apophysis_proximalis
def: "Swelling on the extensor surface of the proximal compound head of the tibiale and fibulare." [AAO:LAP]
relationship: part_of AAO:0000220 ! hind_mesopodium

[Term]
id: AAO:0000917
name: apophysis_distalis_of_tibiale_fibulare
def: "Swelling on the extensor surface of the distal compound head of the tibiale and fibulare." [AAO:LAP]
relationship: part_of AAO:0000220 ! hind_mesopodium

[Term]
id: AAO:0000918
name: tarsal_1
def: "Small element that articulates with the prehallux, metatarsal I and element Y. It may be fused to tarsal 2." [AAO:Fabrezi_1993, AAO:Fancis_1934]
is_a: AAO:0000914 ! distal_tarsal

[Term]
id: AAO:0000919
name: tarsal_2
def: "Small element that articulates anteriorly with metatarsal II. It may be fused to tarsal 1 or to tarsal 3." [AAO:Fabrezi_1993, AAO:Francis_1934]
is_a: AAO:0000914 ! distal_tarsal

[Term]
id: AAO:0000920
name: tarsal_3
def: "Small element that articulates anteriorly with metatarsal III. It may be fused to tarsal 2." [AAO:Fabrezi_1993, AAO:Francis_1934]
is_a: AAO:0000914 ! distal_tarsal

[Term]
id: AAO:0000921
name: element_Y_of_hind_mesopodium
def: "Oval tarsal element that is located on the anteromedial side of the tibiale. Anteriorly, it articulates with the proximal prehallux, tarsals 1, 2, and 3." [AAO:Fabrezi_1993]
relationship: part_of AAO:0000220 ! hind_mesopodium

[Term]
id: AAO:0000922
name: prehallux
def: "One to three or four elements located ventral and medial to the metatarsal of digit I. When more than one elements are present, they are smaller than the proximal prehallux." [AAO:Fabrezi_1993, AAO:Maglia_et_al_2007]
relationship: part_of AAO:0000220 ! hind_mesopodium

[Term]
id: AAO:0000923
name: intermedium
def: "Small, wedge-shaped tarsal element of which the thiner edge projects between the tibia and fibula, thus separating the distal ends of this two bones. Distally, it articulates with the centrale, fibulare, and tibiale." [AAO:Francis_1934]
relationship: part_of AAO:0000220 ! hind_mesopodium

[Term]
id: AAO:0000924
name: centrale
def: "Oval tarsal element that is located on the center of the mesopodium. It articulates with all other elements of the tarsus except tarsal 5." [AAO:Francis_1934]
relationship: part_of AAO:0000220 ! hind_mesopodium

[Term]
id: AAO:0000925
name: metatarsal_I
def: "Dumb-bell-shaped bone of endochondral origin with cartilaginous epiphyses that articulates with the prepollex and tarsal 1 proximally and with the proximal phalanx of digit I distally." [AAO:Fabrezi_1993, AAO:Francis_1934]
relationship: part_of AAO:0000221 ! hind_metapodium

[Term]
id: AAO:0000926
name: metatarsal_II
def: "Dumb-bell-shaped bone of endochondral origin with cartilaginous epiphyses that articulates with tarsal 2 proximally and with the proximal phalanx of digit II distally." [AAO:Fabrezi_1993, AAO:Francis_1934]
relationship: part_of AAO:0000221 ! hind_metapodium

[Term]
id: AAO:0000927
name: metatarsal_III
def: "Dumb-bell-shaped bone of endochondral origin with cartilaginous epiphyses that articulates with tarsal 3 proximally and with the proximal phalanx of digit III distally." [AAO:Fabrezi_1993, AAO:Francis_1934]
relationship: part_of AAO:0000221 ! hind_metapodium

[Term]
id: AAO:0000928
name: metatarsal_IV
def: "Dumb-bell-shaped bone of endochondral origin with cartilaginous epiphyses that articulates with tarsal 4 or the distal head of the tibiale-fibulare proximally and with the proximal phalanx of digit IV distally." [AAO:Fabrezi_1993, AAO:Francis_1934]
relationship: part_of AAO:0000221 ! hind_metapodium

[Term]
id: AAO:0000929
name: metatarsal_V
def: "Dumb-bell-shaped bone of endochondral origin with cartilaginous epiphyses that articulates with tarsal 5 or the distal head of the tibiale-fibulare proximally and with the proximal phalanx of digit V distally." [AAO:Fabrezi_1993, AAO:Francis_1934]
relationship: part_of AAO:0000221 ! hind_metapodium

[Term]
id: AAO:0000930
name: phalanges_of_hind_digit
def: "Dumb-bell shaped bones of endochondral origin with cartilaginous epiphyses that make the five digits of the pes. The terminal phalanges are much smaller than the proximal and penultimate phalanges. The typical phalangeal formula of the pes, in a medial to lateral sequence, is 2(1)-2-3-4(3)-3(2)." [AAO:Francis_1934, AAO:Maglia_et_al_2007]
relationship: part_of AAO:0000888 ! hind_digit

[Term]
id: AAO:0000931
name: intercalary_element_of_hind_digit
def: "Small elements of endochondral origin present in all digits of the pes. Each intercalary element articulates with the anteroventral end of the penultimate phalanx proximally and the distal phalanx distally." [AAO:Maglia_et_al_2007]
relationship: part_of AAO:0000888 ! hind_digit

[Term]
id: AAO:0000932
name: tarsal_4
def: "Small element that articulates anteriorly with metatarsal IV. It may be absent in some taxa." [AAO:Fabrezi_1993]
is_a: AAO:0000914 ! distal_tarsal

[Term]
id: AAO:0000933
name: tarsal_5
def: "Small element that articulates anteriorly with metatarsal V. It may be absent in some taxa." [AAO:Francis_1934]
is_a: AAO:0000914 ! distal_tarsal

[Term]
id: AAO:0000934
name: foramen_perforans_tarsi
def: "Small opening between the centrale and fibulare that allows the perforans tarsi artery to pass from the ventral to the dorsal side of the ankle." [AAO:Francis_1934]
is_a: AAO:0000910 ! hind_limb_opening

[Term]
id: AAO:0000935
name: scapular_area
def: "Dorso-lateral portion of the pectoral girdle." [AAO:Francis_1934]
related_synonym: "pars scapularis" []
related_synonym: "scapula et adscapulum" []
related_synonym: "scapula-suprascapula area" []
related_synonym: "scapulum et episcapulum" []
relationship: part_of AAO:0000754 ! pectoral_girdle_skeleton

[Term]
id: AAO:0000936
name: zonal_element
def: "All those parts of the pectoral girdle in the central region of the zonal area." [AAO:LAP]
relationship: part_of AAO:0000757 ! zonal_area

[Term]
id: AAO:0000937
name: prezonal_element
def: "All those parts of the pectoral girdle that lie anterior to the zonal area." [AAO:LAP]
relationship: part_of AAO:0000757 ! zonal_area

[Term]
id: AAO:0000938
name: postzonal_element
def: "All those parts of the pectoral girdle that lies posterior to the zonal area." [AAO:LAP]
relationship: part_of AAO:0000757 ! zonal_area

[Term]
id: AAO:0000939
name: mesosternum
def: "Proximal portion of the sternum, usually elaborated into a stylum that may be ossified." [AAO:Duellman_and_Trueb_1994]
relationship: part_of AAO:0000765 ! sternum

[Term]
id: AAO:0000940
name: xiphisternum
def: "Distal, cartilaginous portion of the sternum." [AAO:Duellman_and_Trueb_1994]
related_synonym: "metasternum" []
relationship: part_of AAO:0000765 ! sternum

[Term]
id: AAO:0000941
name: arciferal_girdle
def: "Pectoral girdle in which the epicoracoid cartilages are elaborated into posteriorly directed epicoracoid horns. Most arciferal pectoral girdles are characterized by fusion of the epicoracoid cartilages in the interclavicle region. Posterior to the clavicles, the epicoracoids usually are free and overlapping." [AAO:Duellman_and_Trueb_1994, AAO:Griffiths_1959]
is_a: AAO:0000422 ! pectoral_girdle

[Term]
id: AAO:0000942
name: firmisternal_girdle
def: "Pectoral girdle that lacks epicoracoid horns. The sternum is fused to the pectoral arch, and the epicoracoid cartilages of each half of the girdle are fused to one another. The midzonal length of the girdle is shorter than that of an arciferal girdle, but pre- and postzonal elements tend to be longer." [AAO:Duellman_and_Trueb_1994, AAO:Griffiths_1959]
is_a: AAO:0000422 ! pectoral_girdle

[Term]
id: AAO:0000943
name: pseudofirmisternal_girdle
def: "Modified arciferal pectoral girdle in which the fusion of the epicoracoid cartilages in the interclavicle region is extended posteriorly. Thus, the cartilages no longer overlap freely, and functionally a partially firmisternal condition is created." [AAO:Duellman_and_Trueb_1994]
is_a: AAO:0000422 ! pectoral_girdle

[Term]
id: AAO:0000944
name: pseudoarciferal_girdle
def: "Modified firmisternal pectoral girdle in which the epicoracoid cartilages are partly free and overlapping; however, the epicoracoids are fused to one another and the sternum postermodially." [AAO:Duellman_and_Trueb_1994]
is_a: AAO:0000422 ! pectoral_girdle

[Term]
id: AAO:0000945
name: inscriptional_rib
def: "Three pairs of cartilaginous elements posterior to the sternum that lie in the myosepta of the ventral trunk musculature." [AAO:Duellman_and_Trueb_1994]
related_synonym: "abdominal ribs" []
relationship: part_of AAO:0000938 ! postzonal_element

[Term]
id: AAO:0000946
name: fore_metapodium
def: "Segment of the forearm corresponding to the metacarpus, which articulates with the carpals at one end and with the phalanges at the other end." [AAO:Duellman_and_Trueb_1994]
is_a: AAO:0000202 ! forelimb_skeleton

[Term]
id: AAO:0000947
name: phalanges_of_fore_digit
def: "Dumb-bell shaped bones of endochondral origin with cartilaginous epiphyses that make the four digits of the manus. The terminal phalanges are much smaller than the proximal and penultimate phalanges. The typical phalangeal formula of the manus, in a medial to lateral sequence, is 2-2-3-3." [AAO:Maglia_et_al_2007]
relationship: part_of AAO:0000857 ! fore_digit

[Term]
id: AAO:0000948
name: articular_process
def: "Paired processes located on the anterior end of the cricoid cartilage." [AAO:Maglia_et_al_2007]
related_synonym: "processus articularis anterior" []
relationship: part_of AAO:0000675 ! cricoid_cartilage

[Term]
id: AAO:0000949
name: posterior_ramus_of_cleithrum
def: "Laminar subdivision of the cleithrum that extends along the ventral (lateral) midbody of the suprascapula." [AAO:Trueb_1973]
relationship: part_of AAO:0000750 ! cleithrum

[Term]
id: AAO:0000950
name: os_triangulare
def: "Small, broadly triangular bar of bone lying across the ventral side of the pharynx at the junction of the M. genio-hyoideus and the M. rectus cervicis superficialis." [AAO:Francis_1934]
related_synonym: "basi-branchial II" []
related_synonym: "os thyroideum" []
related_synonym: "os triquetum" []
related_synonym: "sternum" []
relationship: part_of AAO:0000682 ! hyoid_apparatus_skeleton

[Term]
id: AAO:0000951
name: anterior_radial
def: "Paired, horn-like processes of basibranchial I that protrude in an antero-dorso-lateral direction, being more or less embedded in the tongue musculature. These elements contitute the hypohyals." [AAO:Francis_1934]
relationship: part_of AAO:0000682 ! hyoid_apparatus_skeleton

[Term]
id: AAO:0000952
name: posterior_radial
def: "Paired, horn-like processes of basibranchial I that protrude in an antero-dorso-lateral direction, being more or less embedded in the tongue musculature. They arise secondarily during metamorphosis, and are therefore not strictly part of the visceral skeleton." [AAO:Francis_1934]
relationship: part_of AAO:0000682 ! hyoid_apparatus_skeleton

[Term]
id: AAO:0000953
name: ceratobranchials_II--IV
def: "Paired bars that articulate with hypobranchial II. Reduction of loss of these elements is common in salamanders." [AAO:LAP]
related_synonym: "epibranchials" []
relationship: part_of AAO:0000682 ! hyoid_apparatus_skeleton

[Term]
id: AAO:0000954
name: hypobranchial_I
def: "Paired bar that articulates with basibranchial I. It forms the anterior portion of the posterior cornu of the hyoid." [AAO:Francis_1934]
relationship: part_of AAO:0000682 ! hyoid_apparatus_skeleton

[Term]
id: AAO:0000955
name: ceratobranchial_I
def: "Paired bar that articulates with, or is fused to, hypobranchial I. It forms the posterior portion of the posterior cornu of the hyoid." [AAO:Francis_1934]
related_synonym: "epibranchial" []
relationship: part_of AAO:0000682 ! hyoid_apparatus_skeleton

[Term]
id: AAO:0000956
name: hypobranchial_II
def: "Paired bar that articulates anteriorly with basibranchial I and posteriorly with ceratobranchials II--IV." [AAO:Duellman_and_Trueb_1994]
relationship: part_of AAO:0000682 ! hyoid_apparatus_skeleton

[Term]
id: AAO:0000957
name: basihyal
def: "Paired, anterior element that articulates medially with basibranchial I and posterolaterally with the paired hypohyals." [AAO:LAP]
relationship: part_of AAO:0000682 ! hyoid_apparatus_skeleton

[Term]
id: AAO:0000958
name: hypohyal
def: "Paired element that articulates anterioly with the basihyal and posteriorly with the ceratohyal hypohyals." [AAO:LAP]
relationship: part_of AAO:0000682 ! hyoid_apparatus_skeleton

[Typedef]
id: develops_from
name: develops_from
is_transitive: true

[Typedef]
id: part_of
name: part_of
is_transitive: true

